<?xml version="1.0" encoding="utf-8"?>

<section xml:id="sec_riemannspere">
  <title>Infinity and the Cross Ratio</title>
  <p>
    In the context of M&#xf6;bius transformations,
    it is useful to introduce a formal way of saying that a function
    <m>f</m>
    <q>blows up</q>
    in absolute value, and this gives rise to a notion of infinity.
    <idx><h>infinity</h></idx>
    <idx><h>limit</h><h>infinity</h></idx>
  </p>
  <definition>
    <statement>
      <p>
        Suppose <m>f: G \to \C</m>.
        <ol marker="(a) ">
          <li>
            <p>
              <m>\lim_{z\to z_0}f(z)=\infty</m> means that for every
              <m>M>0</m> we can find <m>\delta>0</m> so that, 
              for all <m>z\in G</m> satisfying <m>0\lt \abs{z-z_0}\lt
              \delta</m>, 
              we have <m>\abs{f(z)}>M</m>.
            </p>
          </li>
          <li>
            <p>
              <m>\lim_{z\to \infty}f(z)=L</m> means that for every
              <m>\epsilon>0</m> we can find <m>N>0</m> so that,
              for all <m>z\in G</m> satisfying <m>\abs{z}>N</m>,
              we have <m>\abs{f(z)-L}\lt \epsilon</m>.
            </p>
          </li>
          <li>
            <p>
              <m>\lim_{z\to \infty}f(z)=\infty</m> means that for
              every <m>M>0</m> we can find <m>N>0</m> so that, 
              for all <m>z\in G</m> satisfying <m>\abs{z}>N</m>,
              we have <m>\abs{f(z)}>M</m>.
            </p>
          </li>
        </ol>
      </p>
      <p>
        In the first definition we require that <m>z_0</m> be an
        accumulation point of <m>G</m> while in the second and third
        we require that <m>\infty</m> be an 
        <q>extended accumulation point</q>
        of <m>G</m>,
        in the sense that for every <m>B>0</m> there is some <m>z\in
        G</m> with <m>\abs z>B</m>. 
      </p>
    </statement>
  </definition>
  <p>
    As in <xref ref="sec_limitsandcontinuity"/>,
    the limit, in any of these senses, is unique if it exists.
  </p>
  <example>
    <statement>
      <p>
        We claim that <m>\lim_{ z \to 0 } \frac 1 { z^2 } =
        \infty</m>: Given <m>M > 0</m>, 
        let <m>\delta := \frac 1 { \sqrt M }</m>.
        Then <m>0 \lt  |z| \lt  \delta</m> implies
        <me>
          |f(z)| \= \left| \frac 1 { z^2 } \right| \ > \ \frac 1 {
          \delta^2 } \= M \, 
        </me>.
      </p>
    </statement>
  </example>
  <example>
    <statement>
      <p>
        Let <m>f(z) = \frac{ az+b }{ cz+d }</m> be a M&#xf6;bius
        transformation with <m>c \ne 0</m>. 
        Then <m>\lim_{ z \to \infty } f(z) = \frac a c</m>.
      </p>
      <p>
        To simplify the notation, introduce the constant <m>L := |ad
        -bc|</m>. 
        Given <m>\epsilon > 0</m>,
        let <m>N := \frac L { |c|^2 \epsilon } + \left| \frac d c
        \right|</m>. 
        Then <m>|z| > N</m> implies, with the reverse triangle inequality
        (<xref ref="cor_triangleineq"/><xref ref="revtrianineq"/>), 
        that
        <me>
          |cz+d| \ \ge \ \bigl| |c||z| - |d| \bigr| \ \ge \ |c||z| -
          |d| \ > \ \frac L { |c| \epsilon } 
        </me>
        and so
        <me>
          \left| f(z) - \frac a c \right| \= \left| \frac{ c(az+b) -
          a(cz+d) }{ c(cz+d) } \right| \= \frac L { |c| \, |cz+d| } \
          \lt  \ \epsilon \, 
        </me>.
      </p>
    </statement>
  </example>
  <p>
    We stress that <m>\infty</m> is not a number in <m>\C</m>,
    just as <m>\pm \infty</m> are not numbers in <m>\R</m>.
    However, we can <em>extend</em>
    <m>\C</m> by adding on <m>\infty</m>, if we are careful.
    We do so by realizing that we are always talking about a limit
    when handling <m>\infty</m>. 
    It turns out
    (see <xref ref="ex_limitrulesinfty"/>)
    that the usual limit rules behave well when we mix complex numbers
    and <m>\infty</m>. 
    For example, if <m>\lim_{z\to z_0}f(z)=\infty</m> and
    <m>\lim_{z\to z_0}g(z)=a</m> is finite then the usual
    <em>limit of sum = sum of limits</em>
    rule still holds and gives <m>\lim_{z\to
    z_0}(f(z)+g(z))=\infty</m>. 
    The following definition captures the philosophy of this paragraph.
  </p>

  <definition>
    <statement>
      <p>
        The <em>extended complex plane</em>
        is the set <m>\Chat := \C\cup\listset\infty</m>,
        together with the following algebraic properties: For any <m>a
        \in \C</m>, 
        <ol marker="(a) ">
          <li>
            <p>
              <m>\infty+a = a+\infty=\infty</m>
            </p>
          </li>
          <li>
            <p>
              if <m>a \neq 0</m> then <m>\infty\cdot a = a\cdot\infty
              = \infty</m> 
            </p>
          </li>
          <li>
            <p>
              <m>\infty\cdot\infty =\infty</m>
            </p>
          </li>
          <li>
            <p>
              <m>\frac a \infty = 0</m>
            </p>
          </li>
          <li>
            <p>
              if <m>a \neq 0</m> then <m>\frac a 0 = \infty </m>.
            </p>
          </li>
        </ol>
        <idx><h>complex plane</h><h>extended</h></idx>
        <idx><h>extended complex plane</h></idx>
      </p>
      <p>
        The extended complex plane is also called the <em>Riemann
        sphere</em> 
        or the <em>complex projective line</em>,
        denoted <m>\mathbb{CP}^1</m>.
        <idx><h>complex projective line</h></idx>
        <idx><h>Riemann sphere</h></idx>
      </p>
    </statement>
  </definition>
  <p>
    If a calculation involving <m>\infty</m> is not covered by the
    rules above then we must investigate the limit more carefully.
    For example, it may seem strange that <m>\infty+\infty</m> is not
    defined, but if we take the limit of <m>z+(-z)=0</m> as
    <m>z\to\infty</m> we will get <m>0</m>, even though the individual
    limits of <m>z</m> and <m>-z</m> are both<nbsp/><m>\infty</m>.
  </p>
  <p>
    Now we reconsider M&#xf6;bius transformations with <m>\infty</m>
    in mind.  For example, <m>f(z)= \frac 1 z</m> is now defined for
    <m>z=0</m> and <m>z=\infty</m>, with <m>f(0)=\infty</m> and
    <m>f(\infty)=0</m>, and so we might argue the proper domain for
    <m>f(z)</m> is actually <m>\Chat</m>.  Let's consider the other
    basic types of M&#xf6;bius transformations.  A translation <m>f(z)
    = z+b</m> is now defined for <m>z=\infty</m>, with <m>f(\infty) =
    \infty+b = \infty</m>, and a dilation <m>f(z) = az</m> (with
    <m>a\ne0</m>) is also defined for <m>z=\infty</m>, with
    <m>f(\infty) = a\cdot\infty=\infty</m>.  Since every M&#xf6;bius
    transformation can be expressed as a composition of translations,
    dilations and inversions (<xref ref="transdilinv"/>), we see that
    every M&#xf6;bius transformation may be interpreted as a
    transformation of <m>\Chat</m> onto <m>\Chat</m>.  This general
    case is summarized in the following extension of <xref
    ref="inversemobius"/>.
  </p>
  <corollary xml:id="cor_inversemobius">
    <statement>
      <p>
        Suppose <m>ad-bc \ne 0</m> and <m>c \ne 0</m>,
        and consider <m>f: \Chat \to \Chat</m> defined through
        <me>
          f(z) := \begin{cases}\frac{az+b}{cz+d} \amp  \text{ if }  z
          \in \C \setminus \left\{ - \frac d c \right\} , \\ \infty
          \amp  \text{ if }  z = - \frac d c \, , \\ \frac a c \amp
          \text{ if }  z = \infty \, . \end{cases} 
        </me>
      </p>
      <p>
        Then <m>f</m> is a bijection.
      </p>
    </statement>
  </corollary>
  <p>
    This corollary also holds for <m>c = 0</m> if we then define
    <m>f(\infty) = \infty</m>. 
  </p>
  <example xml:id="ex_mobiusinverse3">
    <statement>
      <p>
        Continuing <xref ref="ex_mobiusinverse">Examples</xref> and
        <xref ref="ex_mobiusinverse2"></xref>, consider once more the
        M&#xf6;bius transformation <m>f(z) = \frac{ z-1 }{ iz+i }</m>.
        With the definitions <m>f(-1) = \infty</m> and <m>f(\infty) =
        -i</m>, we can extend <m>f</m> to a function <m>\Chat \to
        \Chat</m>. 
      </p>
    </statement>
  </example>
  <p>
    With <m>\infty</m> on our mind we can also add some insight to
    <xref ref="circlestocircles"/>.  We recall that in
    <xref ref="ex_mobiusinverse2"/>, we proved that
    <m>f(z) = \frac{ z-1 }{ iz+i }</m> maps the unit circle to the
    real line.  Essentially the same proof shows that, more generally,
    any circle passing through <m>-1</m> gets mapped to a line (see
    <xref ref="exercise_mobiusinverse2"/>).  The
    original domain of <m>f</m> was <m>\C \setminus \{ -1 \}</m>, so
    the point <m>z = -1</m> must be excluded from these circles.
    However, by thinking of <m>f</m> as function from <m>\Chat</m> to
    <m>\Chat</m>, we can put <m>z = -1</m> back into the picture, and
    so <m>f</m> transforms circles that pass through <m>-1</m> to
    straight lines <em>plus</em> <m>\infty</m>.  If we remember that
    <m>\infty</m> corresponds to being arbitrarily far away from any
    point in <m>\C</m>, we can visualize a line plus <m>\infty</m> as
    a circle passing through <m>\infty</m>.  If we make this a
    definition, then <xref ref="circlestocircles"/> can
    be expressed as: <em>any M&#xf6;bius transformation of
    <m>\Chat</m> transforms circles to circles</em>.
  </p>
  <p>
    We can take this remark a step further, based on the idea that
    three distinct points in <m>\Chat</m> determine a unique circle
    passing through them: If the three points are in <m>\C</m> and
    nonlinear, this fact comes straight from Euclidean geometry; if
    the three points are on a straight line or if one of the points is
    <m>\infty</m>, then the circle is a straight line plus
    <m>\infty</m>.
  </p>
  <example>
    <statement>
      <p>
        The M&#xf6;bius transformation <m>f: \Chat \to \Chat</m> given
        by <m>f(z) = \frac{ z-1 }{ iz+i }</m> maps
        <me>
          1 \mapsto 0 \, , \qquad \qquad i \mapsto 1 \, , \qquad
          \text{ and }  \qquad -1 \mapsto \infty \, 
        </me>.
      </p>
      <p>
        The points <m>1</m>, <m>i</m>, and <m>-1</m> uniquely
        determine the unit circle and the points 0, 1, and
        <m>\infty</m> uniquely determine the real line, viewed as a
        circle in <m>\Chat</m>.  Thus <xref
        ref="cor_inversemobius"/> implies that <m>f</m>
        maps the unit circle to <m>\R</m>, which we already concluded
        in <xref ref="ex_mobiusinverse2"/>.
      </p>
    </statement>
  </example>
  <p>
    Conversely, if we know where three distinct points in <m>\Chat</m>
    are transformed by a M&#xf6;bius transformation then we should be
    able to figure out everything about the transformation.  There is
    a computational device that makes this easier to see.
  </p>
  <definition>
    <statement>
      <p>
        If <m>z</m>, <m>z_1</m>, <m>z_2</m>, and <m>z_3</m> are any
        four points in <m>\Chat</m> with <m>z_1</m>, <m>z_2</m>, and
        <m>z_3</m> distinct, then their <em>cross ratio</em>
        is defined as
        <me>
          [z,z_1,z_2,z_3] \ := \ \frac{(z-z_1)(z_2-z_3)}{(z-z_3)(z_2-z_1)} \,
        </me>.
        <idx><h>cross ratio</h></idx>
      </p>
      <p>
        This includes the implicit definitions <m>[z_3,z_1,z_2,z_3] =
        \infty</m> and, 
        if one of <m>z</m>, <m>z_1</m>, <m>z_2</m>,
        or <m>z_3</m> is <m>\infty</m>,
        then the two terms containing <m>\infty</m> are canceled;
        e.g., <m>[z,\infty, z_2, z_3] = \frac{ z_2 - z_3 }{ z - z_3 }</m>.
      </p>
    </statement>
  </definition>
  <example>
    <statement>
      <p>
        Our running example <m>f(z) = \frac{ z-1 }{ iz+i }</m> can be
        written as <m>f(z) = [z,1,i,-1]</m>.
      </p>
    </statement>
  </example>
  <proposition xml:id="crossratio">
    <statement>
      <p>
        The function <m>f: \Chat \to \Chat</m> defined by
        <m>f(z)=[z,z_1,z_2,z_3]</m> is a M&#xf6;bius transformation
        that satisfies
        <me>
          f(z_1) = 0 \, ,\qquad f(z_2) = 1 \, ,\qquad f(z_3)= \infty \,
        </me>.
      </p>
      <p>
        Moreover, if <m>g</m> is any M&#xf6;bius transformation with
        <m>g(z_1) = 0</m>, <m>g(z_2) = 1</m>, and <m>g(z_3)=
        \infty</m>, then <m>f</m> and <m>g</m> are identical.
      </p>
    </statement>
    <proof>
      <p>
        Most of this follows from our definition of <m>\infty</m>,
        but we need to prove the uniqueness statement.
        By <xref ref="inversemobius">Proposition</xref>,
        the inverse <m>f^{-1}</m> is a M&#xf6;bius transformation and,
        by <xref ref="ex_mobiusgroup">Exercise</xref>,
        the composition <m>h := g\circ f^{-1}</m> is again a
        M&#xf6;bius transformation. 
        Note that <m>h(0) = g(f^{-1}(0)) = g(z_1) = 0</m> and,
        similarly, <m>h(1) = 1</m> and <m>h(\infty) = \infty</m>.
        If we write <m>h(z)=\frac{az+b}{cz+d}</m> then
        <md>
          <mrow>0 \= h(0) \= \frac bd \amp  \implies  b=0</mrow>
          <mrow>\infty \= h(\infty) \= \frac ac \amp  \implies
          c=0</mrow>
          <mrow>1 \= h(1) \= \frac{a+b}{c+d} \= \frac {a+0}{0+d} \=
          \frac ad \amp  \implies  a=d</mrow>
        </md>
        and so
        <me>
          h(z)\=\frac{az+b}{cz+d} \= \frac{az+0}{0+d} \= \frac ad \, z
          \= z \, 
        </me>,
        the identity function.
        But since <m>h = g\circ f^{-1}</m>,
        this means that <m>f</m> and <m>g</m> are identical.
      </p>
    </proof>
  </proposition>
  <p>
    So if we want to map three given points of <m>\Chat</m> to
    <m>0</m>, <m>1</m> and <m>\infty</m> by a M&#xf6;bius
    transformation, then the cross ratio gives us the only way to do
    it.  What if we have three points <m>z_1</m>, <m>z_2</m> and
    <m>z_3</m> and we want to map them to three other points
    <m>w_1</m>, <m>w_2</m> and <m>w_3</m>?
  </p>
  <corollary>
    <statement>
      <p>
        Suppose <m>z_1</m>, <m>z_2</m> and <m>z_3</m> are distinct
        points in <m>\Chat</m> and <m>w_1</m>, <m>w_2</m> and
        <m>w_3</m> are distinct points in <m>\Chat</m>.  Then there is
        a unique M&#xf6;bius transformation <m>h</m> satisfying
        <m>h(z_1)=w_1</m>, <m>h(z_2)=w_2</m>, and <m>h(z_3)=w_3</m>.
      </p>
    </statement>
    <proof>
      <p>
        Let <m>h=g^{-1}\circ f</m> where
        <m>f(z)=[z,z_1,z_2,z_3]</m> and <m>g(w)=[w,w_1,w_2,w_3]</m>.
        Uniqueness follows as in the proof of
        <xref ref="crossratio"/>.
      </p>
    </proof>
  </corollary>
  <p>
    This theorem gives an explicit way to determine <m>h</m> from the
    points <m>z_j</m> and <m>w_j</m> but, in practice, it is often
    easier to determine <m>h</m> directly from the conditions
    <m>f(z_j)=w_j</m> (by solving for <m>a</m>, <m>b</m>, <m>c</m> and
    <m>d</m>).
  </p>
</section>
