<?xml version="1.0" encoding="utf-8"?>

<section xmlns:xi="http://www.w3.org/2001/XInclude"
         xml:id="sec_mobius">
  <title>M&#xf6;bius Transformations</title>
  <p>
    <idx><h>Mobius transformation@M&#xf6;bius transformation</h></idx>
  </p>
  <p>
    The first class of functions that we will discuss in some detail
    are built from linear polynomials.
  </p>

  <definition>
    <statement>
      <p>
        A <em>linear fractional transformation</em>
        is a function of the form
        <me>
          f(z) \ = \ \frac{ az+b }{ cz+d }
        </me>
        where <m>a,b,c,d \in \C</m>.
        <idx><h>linear fractional transformation</h></idx> 
        If <m>ad-bc \not= 0</m> then <m>f</m> is called a
        <em>M&#xf6;bius<fn> 
        Named after August Ferdinand M&#xf6;bius
        (1790<ndash/>1868). 
        </fn> transformation</em>.
      </p>
    </statement>
  </definition>
  
  <p>
    <xref ref="polynomialsholomorphic"/>
    said that any polynomial in <m>z</m> is an entire function,
    and so the linear fractional transformation
    <m>f(z) = \frac{ az+b }{ cz+d }</m> is holomorphic in <m>\C
    \setminus \{ - \frac d c \}</m>, 
    unless <m>c=0</m>
    (in which case <m>f</m> is entire).
    If <m>c \ne 0</m> then <m>\frac{ az+b }{ cz+d } = \frac a c</m>
    implies <m>ad-bc = 0</m>, 
    which means that a M&#xf6;bius transformation
    <m>f(z) = \frac{ az+b }{ cz+d }</m> will never take on the value
    <m>\frac a c</m>. 
    Our first proposition in this chapter says that with these small
    observations about the domain and image of a M&#xf6;bius
    transformation, 
    we obtain a class of bijections,
    which are quite special among complex functions.
    <idx><h>bijection</h></idx>
  </p>
  <p>
    <idx><h>inverse function</h><h>of a M&#xf6;bius transformation</h></idx>
  </p>
  <proposition xml:id="inversemobius">
    <statement>
      <p>
        Let <m>a,b,c,d \in \C</m> with <m>c \ne 0</m>.  Then <m>f: \C
        \setminus \{ - \frac d c \} \to \C \setminus \{ \frac a c
        \}</m> given by <m>f(z) = \frac{ az+b }{ cz+d }</m> has the
        inverse function <m>f^{-1}: \C \setminus \{ \frac a c \} \to
        \C \setminus \{ - \frac d c \}</m> given by
        <me>
          f^{-1} (z) \ = \ \frac{ dz-b }{ -cz+a } \,
        </me>.
      </p>
    </statement>
  </proposition>
  <p>
    We remark that the same formula for <m>f^{-1} (z)</m> works when
    <m>c = 0</m>, except that in this case both domain and image of
    <m>f</m> are <m>\C</m>; see <xref ref="ex_inversemobisc_0"/>.
    In either case, we note
    that the inverse of a M&#xf6;bius transformation is another
    M&#xf6;bius transformation.
  </p>
  <example xml:id="ex_mobiusinverse">
    <statement>
      <p>
        Consider the linear fractional transformation <m>f(z) = \frac{
        z-1 }{ iz+i }</m>.  This is a M&#xf6;bius transformation
        (check the condition!)  with domain <m>\C \setminus \{ -1
        \}</m> whose inverse can be computed via
        <me>
          \frac{ z-1 }{ iz+i } \ = \ w \qquad \Longleftrightarrow \qquad
          z \ = \ \frac{ iw + 1 }{ -iw + 1 } \, 
        </me>,
        so that <m>f^{-1} (z) = \frac{ iz + 1 }{ -iz + 1 }</m>,
        with domain <m>\C \setminus \{ -i \}</m>.
      </p>
    </statement>
  </example>
  <proof>
    <p>
      We first prove that <m>f</m> is one-to-one.
      If <m>f(z_1) = f(z_2)</m>, that is,
      <me>
        \frac{ az_1+b }{ cz_1+d } \ = \ \frac{ az_2+b }{ cz_2+d } \,
      </me>,
      then <m>(az_1+b)(cz_2+d) = (az_2+b)(cz_1+d)</m>,
      which can be rearranged to
      <me>
        (ad-bc)(z_1-z_2) \ = \ 0 \,
      </me>.
    </p>
    <p>
      Since <m>ad-bc \not= 0</m> this implies that <m>z_1 = z_2</m>.
      This shows that <m>f</m> is one-to-one.
    </p>
    <p>
      <xref ref="prob_mobiusinverse"/>
      verifies that the M&#xf6;bius transformation
      <m>g(z) = \frac{ dz-b }{ -cz+a }</m> is the inverse of <m>f</m>,
      and by what we have just proved,
      <m>g</m> is also one-to-one.
      But this implies that <m>f: \C \setminus \{ - \frac d c \} \to
      \C \setminus \{ \frac a c \}</m> is onto. 
    </p>
  </proof>
  <p>
    We remark that M&#xf6;bius transformations provide an immediate
    application of <xref ref="dernonzeroconformal">Proposition</xref>, 
    as the derivative of <m>f(z) = \frac{ az+b }{ cz+d }</m> is
    <me>
      f'(z) \ = \ \frac{ a(cz+d) - c(az+b) }{ (cz+d)^2 } \ = \ \frac{ ad -
      bc }{ (cz+d)^2 } 
    </me>
    and thus never zero.
    <xref ref="dernonzeroconformal">Proposition</xref>
    implies that M&#xf6;bius transformations are conformal,
        <idx><h>conformal</h></idx>
    that is, they preserve angles.
        <idx><h>function</h><h>conformal</h></idx>
  </p>
  <p>
    M&#xf6;bius transformations have even more fascinating geometric properties.
    En route to an example of such,
    we introduce some terminology.
    Special cases of M&#xf6;bius transformations are <em>translations</em>
    <m>f(z) = z + b</m>, <em>dilations</em>
    <m>f(z) = az</m>, and <em>inversion</em>
    <m>f(z) = \frac 1 z</m>.
        <idx><h>translation</h></idx>
        <idx><h>dilation</h></idx>
        <idx><h>inversion</h></idx>
    The next result says that if we understand those three special
    M&#xf6;bius transformations, 
    we understand them all.
  </p>
  <proposition xml:id="transdilinv">
    <statement>
      <p>
        Suppose <m>f(z) = \frac{ az+b }{ cz+d }</m> is a linear
        fractional transformation. 
        If <m>c=0</m> then
        <me>
          f(z) \ = \ \frac a d \, z + \frac b d \,
        </me>,
        and if <m>c \not= 0</m> then
        <me>
          f(z) \ = \ \frac{ bc-ad }{ c^2 } \frac 1 {z + \frac d c} +
          \frac a c \, 
        </me>.
      </p>
      <p>
        In particular, every linear fractional transformation is a
        composition of translations, dilations, and inversions.
      </p>
    </statement>
  </proposition>
  <proof>
    <p>
      Simplify.
    </p>
  </proof>
  <theorem xml:id="circlestocircles">
    <statement>
      <p>
        M&#xf6;bius transformations map circles and lines into circles
        and lines. 
      </p>
    </statement>
  </theorem>
  <example xml:id="ex_mobiusinverse2">
    <statement>
      <p>
        Continuing <xref ref="ex_mobiusinverse">Example</xref>,
        consider again <m>f(z) = \frac{ z-1 }{ iz+i }</m>.
        For <m>\phi \in \R</m>,
        <md>
          <mrow>
            f(e^{ i \phi }) \amp \ = \ \frac{ e^{ i \phi } - 1 }{ i \,
            e^{ i \phi } + i } \ = \ \frac{ \left( e^{ i \phi } - 1 \right)
            \left( e^{ -i \phi } + 1 \right) }{ i \left| e^{ i \phi } +
            1 \right|^2 }
          </mrow>
          <mrow>
            \amp \ = \ \frac{ e^{ i \phi } - e^{ -i \phi } }{ i
            \left| e^{ i \phi } + 1 \right|^2 } \ = \ \frac{ 2 \Im \left(
            e^{ i \phi } \right) }{ \left| e^{ i \phi } + 1 \right|^2 }
            \ = \ \frac{ 2 \sin \phi }{ \left| e^{ i \phi } + 1 \right|^2 }
          </mrow>
        </md>,
        which is a real number.
        Thus <xref ref="circlestocircles">Theorem</xref>
        implies that <m>f</m> maps the unit circle to the real
        line.
      </p>
    </statement>
  </example>
  <proof>
    <p>
      Translations and dilations certainly map circles and lines into
      circles and lines, 
      so by <xref ref="transdilinv">Proposition</xref>,
      we only have to prove the statement of the theorem for the
      inversion <m>f(z) = \frac 1 z</m>. 
    </p>
    <p>
      The equation for a circle centered at
      <m>x_0 + iy_0</m> with radius <m>r</m> is
      <m>(x-x_0)^2 + (y-y_0)^2 = r^2</m>, which we can transform to
      <men xml:id="eq_circle">
        \alpha (x^2 + y^2) + \beta x + \gamma y + \delta \ = \ 0
      </men>
      for some real numbers <m>\alpha</m>,
      <m>\beta</m>, <m>\gamma</m>,
      and <m>\delta</m> that satisfy <m>\beta^2 + \gamma^2 > 4 \,
      \alpha \delta</m> 
      (see <xref ref="ex_circlegenau"/>).
      The form <xref ref="eq_circle"/> is more convenient for us,
      because it includes the possibility that the equation describes a line
      (precisely when <m>\alpha = 0</m>).
    </p>
    <p>
      Suppose <m>z = x+iy</m> satisfies <xref ref="eq_circle"/>;
      we need to prove that <m>u+iv := \frac 1 z</m> satisfies a
      similar equation. 
      Since
      <me>
        u + iv \ = \ \frac{ x - iy }{ x^2 + y^2 } \,
      </me>,
      we can rewrite <xref ref="eq_circle"/> as
      <md>
        <mrow>
          0 \amp \ = \ \alpha + \beta \frac{ x }{ x^2 + y^2 } +
          \gamma \frac{ y }{ x^2 + y^2 } + \frac \delta { x^2 + y^2 }
        </mrow>
        <mrow xml:id="eq_circleimage" number="yes">
          \amp \ = \ \alpha + \beta u - \gamma v + \delta (u^2 + v^2) \,
        </mrow>
      </md>.
    </p>
    <p>
      But this equation,
      in conjunction with <xref ref="ex_circlegenau"/>,
      says that <m>u+iv</m> lies on a circle or line.
    </p>
  </proof>

  <p>
    <xref ref="fig-inversion"/> demonstrates the effect that the
    inversion <m>f(z)=\frac1z</m> has on horizontal and vertical
    lines.  In particular, the vertical line defined by
    <m>\Re(z)=x_0</m> is mapped into the circle of radius
    <m>\frac1{2x_0}</m> centered at
    <m>\left(\frac1{2x_0},0\right)</m>. 
  </p>
  <figure xml:id="fig-inversion">
    <caption>
      Inversion maps vertical lines, shown on the left, into the
      circles centered on the real axis.  Horizontal lines are mapped
      into circles centered on the imaginary axis.
    </caption>
    <sidebyside widths="48% 48%">
      <image width="100%">
        <prefigure xmlns="https://prefigure.org"
                   label="inversion-domain">
          <xi:include href="prefigure/inversion-domain.xml"/>
        </prefigure>
      </image>
      <image width="100%">
        <prefigure xmlns="https://prefigure.org"
                   label="inversion-codomain">
          <xi:include href="prefigure/inversion-codomain.xml"/>
        </prefigure>
      </image>
    </sidebyside>
  </figure>
</section>
