<?xml version="1.0" encoding="utf-8"?>

<section xml:id="sec_regionsconvergence">
  <title>Regions of Convergence</title>
  <p>
    For the remainder of this chapter (indeed,
    this book) we concentrate on some very special series of functions.
  </p>
  <definition>
    <statement>
      <p>
        A <em>power series
        centered at <m>z_0</m></em> is a series of the form
        <me>
          \s c_k \left( z - z_0 \right)^k
        </me>
        where <m>c_0, c_1, c_2, \ldots \in \C</m>.
        <idx><h>power series</h></idx>
      </p>
    </statement>
  </definition>
  <example>
    <statement>
      <p>
        A slight modification of
        <xref ref="ex_geomseriesasfunction"/>
        gives a fundamental power series,
        namely the <em>geometric series</em>
        <me>
          \sum_{ k \ge 0 } z^k \ = \ \frac 1 {1-z} \,
        </me>.
      </p>
      <p>
        So here <m>z_0 = 0</m> and <m>c_k = 1</m> for all <m>k \ge 0</m>.
        We note that,
        as in <xref ref="ex_geomseriesasfunction"/>,
        this power series converges absolutely for
        <m>|z| \lt 1</m> and uniformly for <m>|z| \le r</m>,
        for any fixed <m>r\lt 1</m>.
        Finally, as in <xref ref="ex_geomseriesdiv"/>,
        the geometric series <m>\sum_{ k \ge 0 } z^k</m> diverges for
        <m>|z| \ge 1</m>. 
      </p>
    </statement>
  </example>
  <p>
    A general power series has a very similar convergence behavior which,
    in fact, comes from comparing it to a geometric series.
  </p>
  <theorem xml:id="convergenceradius">
    <statement>
      <p>
        Given a power series <m>\s c_k ( z - z_0)^k</m>,
        there exists a real number <m>R \ge 0</m> or <m>R = \infty</m>,
        such that
        <ol marker="(a) ">
          <li>
            <p>
              <m>\s c_k ( z - z_0)^k</m> converges absolutely for
              <m>|z-z_0| \lt R</m>; 
            </p>
          </li>
          <li>
            <p>
              <m>\s c_k ( z - z_0)^k</m> converges absolutely and
              uniformly for 
              <m>|z-z_0| \le r</m>, for any <m>r \lt R</m>;
            </p>
          </li>
          <li>
            <p>
              <m>\s c_k ( z - z_0)^k</m> diverges for <m>|z-z_0| > R</m>.
            </p>
          </li>
        </ol>
      </p>
    </statement>
  </theorem>
  <p>
    We remark that this theorem says nothing about the
    convergence/divergence of 
    <m>\s c_k ( z - z_0)^k</m> for <m>|z-z_0| = R</m>.
  </p>
  <definition>
    <statement>
      <p>
        The number <m>R</m> in <xref ref="convergenceradius"/>
        is called the <em>radius of convergence</em>
        of <m>\s c_k ( z - z_0)^k</m>.
        The open disk <m>D[z_0,R]</m> in which the power series
        converges absolutely is the 
        <em>region of convergence</em>.
        (If <m>R=\infty</m> then this is <m>\C</m>.)
        <idx><h>region</h><h>of convergence</h></idx>
      </p>
    </statement>
  </definition>
  <p>
    In preparation for the proof of
    <xref ref="convergenceradius"/>,
    we start with the following observation.
  </p>
  <proposition xml:id="prop_convergenceradius">
    <statement>
      <p>
        If <m>\s c_k ( w - z_0)^k</m> converges, then
        <m>\s c_k ( z - z_0)^k</m> converges absolutely whenever <m>|z
        - z_0| \lt |w - z_0|</m>. 
      </p>
    </statement>
  </proposition>
    <proof>
      <p>
        Let <m>r := |w - z_0|</m>.
        If <m>\s c_k ( w - z_0)^k</m> converges then
        <m>\lim_{ k \to \infty } c_k ( w - z_0)^k = 0</m> and so this
        sequence of terms is bounded 
        (by <xref ref="ex_convseqbounded"/>),
        say
        <me>
          \left| c_k ( w - z_0)^k \right| \ = \ |c_k| \, r^k \ \le \ M \,
        </me>.
      </p>
      <p>
        Now if <m>|z - z_0| \lt  |w - z_0|</m>, then
      <me>
        \s \left| c_k ( z - z_0)^k \right| \ = \ \s |c_k| \, r^k \left(
        \frac{ |z-z_0| }{ r } \right)^k \ \le \ M \s \left( \frac{
        |z-z_0| }{ r } \right)^k 
      </me>.
    </p>
    <p>
      The sum on the right-hand side is a convergent geometric sequence,
      since <m>|z-z_0| \lt r</m>,
      and so <m>\s c_k ( z - z_0)^k</m> converges absolutely by
      <xref ref="cor_comparisonseries"/>.
    </p>
    </proof>
    <p>
      With this preparation, we can now prove <xref ref="convergenceradius"/>.
    </p>
  <proof>
    <p>
      Consider the set
      <me>
        S \ := \ \left\{ x \in \R_{ \ge 0 } : \, \s c_k \, x^k \text{
        converges }  \right\} 
      </me>.
    </p>
    <p>
      (This set is nonempty since <m>0 \in S</m>.)
    </p>
    <p>
      If <m>S</m> is unbounded then
      <m>\s c_k ( z - z_0)^k</m> converges absolutely and uniformly
      for <m>|z-z_0| \le r</m>, 
      for any <m>r</m> (and so this gives the
      <m>R = \infty</m> case of <xref ref="convergenceradius"/>):
      choose <m>x \in S</m> with <m>x > r</m>,
      then <xref ref="prop_convergenceradius"/>
      says that <m>\s c_k \, r^k</m> converges absolutely.
      Since <m>\left| c_k ( z - z_0)^k \right| \le |c_k| r^k</m>,
      we can now use <xref ref="mtest"/>.
    </p>
    <p>
      If <m>S</m> is bounded, let <m>R</m> be its least upper bound.
      <idx><h>least upper bound</h></idx>
      If <m>R = 0</m> then <m>\s c_k ( z - z_0)^k</m> converges only
      for <m>z = z_0</m>, 
      which establishes
      <xref ref="convergenceradius"/> in this case.
    </p>
    <p>
      Now assume <m>R > 0</m>.
      If <m>|z-z_0| \lt  R</m> then
      (because <m>R</m> is a least upper bound for <m>S</m>)
      there exists <m>r \in S</m> such that
      <me>
        |z-z_0| \lt  r \le R \,
      </me>.
    </p>
    <p>
      Thus <m>\s c_k ( w - z_0)^k</m> converges for <m>w=z_0+r</m>,
      and so <m>\s c_k ( z - z_0)^k</m> converges absolutely by
      <xref ref="prop_convergenceradius"/>.
      This finishes (a).
    </p>
    <p>
      If <m>|z-z_0| \le r</m> for some <m>r \lt R</m>,
      again we can find <m>x \in S</m> such that <m>r \lt x \le R</m>.
      Then <m>\s |c_k| \, r^k</m> converges by
      <xref ref="prop_convergenceradius"/>,
      and so <m>\s c_k ( z - z_0)^k</m> converges absolutely and
      uniformly for 
      <m>|z-z_0|\le r</m> by <xref ref="mtest"/>.
      This proves (b).
    </p>
    <p>
      Finally, if <m>|z-z_0| > R</m> then there exists <m>r \notin
      S</m> such that 
      <me>
        R \le r \lt  |z-z_0| \,
      </me>.
    </p>
    <p>
      But <m>\s c_k \, r^k</m> diverges, so
      (by the contrapositive of <xref ref="absconvthm"/>)
      <m>\s |c_k| \, r^k</m> diverges, and so
      (by the contrapositive of <xref ref="prop_convergenceradius"/>)
      <m>\s c_k ( z - z_0)^k</m> diverges, which finishes (c).
    </p>
  </proof>
  <corollary xml:id="cor_roottest">
    <statement>
      <p>
        If <m>\lim_{ k \to \infty } \sqrt[k]{ |c_k| }</m> exists then
        the radius of convergence of <m>\s c_k ( z - z_0)^k</m> equals 
        <me>
          R = \begin{cases}\infty \amp  \text{ if }  \lim_{ k \to
          \infty } \sqrt[k]{ |c_k| } = 0 \, , \\ \frac{ 1 }{ \lim_{ k
          \to \infty } \sqrt[k]{ |c_k| } } \amp  \text{ otherwise. }
          \end{cases} 
        </me>
      </p>
    </statement>
    <proof>
      <p>
        We treat the case that <m>R</m> is finite and leave the case
        <m>R = \infty</m> to <xref ref="ex_roottestRinfty"/>.
      </p>
      <p>
        Given <m>R</m> as in the statement of the corollary, it suffices
        (by <xref ref="convergenceradius"/>)
        to show that <m>\s c_k ( z - z_0)^k</m> converges for
        <m>|z-z_0| \lt R</m> and diverges for <m>|z-z_0| > R</m>.
      </p>
      <p>
        Suppose <m>r := |z-z_0| \lt  R</m>.
        Since <m>\lim_{ k \to \infty } \sqrt[k]{ |c_k| } = \frac 1
        R</m> and <m>\frac{ 2 }{ R+r } > \frac 1 R</m>, 
        there exists <m>N</m> such that <m>\sqrt[k]{ |c_k| } \lt  \frac{
        2 }{ R+r }</m> for <m>k \ge N</m>. 
        For those <m>k</m> we then have
        <me>
          \left| c_k (z-z_0)^k \right| \ = \ |c_k| |z-z_0|^k \ = \ \left(
          \sqrt[k]{ |c_k| } \, r \right)^k \ \lt  \ \left( \frac{ 2r
          }{ R+r } \right)^k 
        </me>
        and so <m>\sum_{ k=N }^\infty c_k (z-z_0)^k</m> converges
        (absolutely) by <xref ref="mtest"/>,
        because <m>\frac{ 2r }{ R+r } \lt 1</m> and thus
        <m>\s \left( \frac{ 2r }{ R+r } \right)^k</m> converges as a
        geometric series. 
        Thus <m>\s c_k (z-z_0)^k</m> converges.
      </p>
      <p>
        Now suppose <m>r = |z-z_0| > R</m>.
        Again because <m>\lim_{ k \to \infty } \sqrt[k]{ |c_k| } =
        \frac 1 R</m> and now <m>\frac{ 2 }{ R+r } \lt  \frac 1 R</m>, 
        there exists <m>N</m> such that <m>\sqrt[k]{ |c_k| } > \frac{
        2 }{ R+r }</m> for <m>k \ge N</m>. 
        For those <m>k</m>,
        <me>
          \left| c_k (z-z_0)^k \right| \ = \ \left( \sqrt[k]{ |c_k| } \,
          r \right)^k \ > \ \left( \frac{ 2r }{ R+r } \right)^k \ > \
          1 \, 
        </me>,
        and so the sequence <m>c_k (z-z_0)^k</m> cannot converge to 0.
        Subsequently
        (by <xref ref="cor_divtest"/>),
        <m>\s c_k (z-z_0)^k</m> diverges.
      </p>
    </proof>
  </corollary>
  <p>
    You might remember this corollary from calculus,
    where it goes by the name <em>root test</em>.
    <idx><h>root test</h></idx>
    Its twin sister, the <em>ratio test</em>,
    is the subject of <xref ref="ex_ratiotest"/>.
  </p>
  <example>
    <statement>
      <p>
        For the power series <m>\ds \s k \, z^k</m> we compute
        <me>
          \lim_{ k \to \infty } \sqrt[k]{ |c_k| } \ = \ \lim_{ k \to
          \infty } \sqrt[k]{ k } \ = \ \lim_{ k \to \infty } e^{ \frac 1
          k \ln(k) } \ = \ e^{ \lim_{ k \to \infty } \frac { \ln(k) } k }
          \ = \ e^0 \ = \ 1 \, 
        </me>,
        and <xref ref="cor_roottest"/>
        gives the radius of convergence 1. (Alternatively, 
        we can argue by differentiating the geometric series.)
      </p>
    </statement>
  </example>
  <example xml:id="exponentialfunctionradius">
    <statement>
      <p>
        Consider the power series <m>\ds \sum_{ k \ge 0 } \frac{ 1 }{
        k! } \, z^k </m>. 
        Since
        <me>
          \lim_{ k \to \infty } \left| \frac{ c_{ k+1 } }{ c_{ k } }
          \right| \ = \ \lim_{ k \to \infty } \frac{ k! }{ (k+1)! } \ = \
          \lim_{ k \to \infty } \frac{ 1 }{ k+1 } \ = \ 0 \, 
        </me>,
        the ratio test
        (<xref ref="ex_ratiotest"/>)
        implies that the radius of convergence of <m>\sum_{ k \ge 0 }
        \frac{ 1 }{ k! } \, z^k</m> is <m>\infty</m>, 
        and so the power series converges absolutely in <m>\C</m>.
        <fn>
          In the next chapter,
          we will see that this power series represents the
          exponential function. 
        </fn>
      </p>
    </statement>
  </example>
  <p>
    By way of <xref ref="sequencecontionuos"/>,
    <xref ref="convergenceradius"/>
    almost immediately implies the following.
  </p>
  <corollary xml:id="powseriescontinuous">
    <statement>
      <p>
        Suppose the power series <m>\s c_k ( z - z_0 )^k</m> has
        radius of convergence <m>R>0</m>. 
        Then the series represents a function that is continuous on
        <m>D[z_0, R]</m>. 
      </p>
    </statement>
  </corollary>
  <proof>
    <p>
      Given any point <m>w \in D[z_0, R]</m>,
      we can find <m>r\lt R</m> such that <m>w \in D[z_0, r]</m>
      (e.g., if 
      <m>R\ne\infty</m> then <m>r = \frac{ |w-z_0| + R }{ 2 }</m> will
      do the trick). 
      <xref ref="convergenceradius"/>
      says that <m>\s c_k ( z - z_0 )^k</m> converges uniformly in
      <m>D[z_0, r]</m>, 
      and so <xref ref="sequencecontionuos"/>
      implies that the power series is continuous in <m>D[z_0, r]</m>,
      and so particularly at <m>w</m>.
    </p>
  </proof>
  <p>
    Finally, mixing <xref ref="seriesintegral"/>
    with <xref ref="convergenceradius"/> gives:
  </p>
  <corollary xml:id="powseriesintegral">
    <statement>
      <p>
        Suppose the power series <m>\s c_k ( z - z_0 )^k</m> has
        radius of convergence <m>R>0</m> and <m>\gamma</m> is a
        piecewise smooth path in <m>D[z_0, R]</m>. 
        <idx><h>power series</h><h>integration of</h></idx>
        Then
        <me>
          \int_\gamma \ \s c_k ( z - z_0 )^k \, \diff{z} \ = \ \s c_k
          \int_\gamma ( z - z_0 )^k \, \diff{z} \, 
        </me>.
      </p>
      <p>
        In particular,
        if <m>\gg</m> is closed then <m>\ds \int_\gg \ \s c_k ( z -
        z_0 )^k \, \diff{z} \ = \ 0 </m>. 
      </p>
    </statement>
  </corollary>
  <proof>
    <p>
      Let <m>r := \max_{ z \in \gg } \left| \gamma(z) -z_0 \right|</m>
      (whose existence is guaranteed by <xref ref="realEVT"/>).
      Then <m>\gg \subset \overline D[z_0, r]</m> and <m>r\lt R</m>.
      <xref ref="convergenceradius"/>
      says that <m>\s c_k \left( z - z_0 \right)^k</m> converges
      uniformly in <m>\overline D[z_0, r]</m>, 
      and so <xref ref="seriesintegral"/>
      allows us to switch integral and summation.
    </p>
    <p>
      The last statement follows now with
      <xref ref="ex_laurentoutlook"/>.
    </p>
  </proof>
  <p>
    These corollaries will become extremely useful in the next chapter.
  </p>
</section>
