<?xml version="1.0" encoding="utf-8"?>

<section xml:id="sec_series"
         xmlns:xi="http://www.w3.org/2001/XInclude">
  <title>Series</title>
  <definition>
    <statement>
      <p>
        A <em>series</em>
        is a sequence <m>\left( a_n \right)</m> whose members are of
        the form
        <m>a_n = \sum_{k=1}^n b_k</m> (or <m>a_n = \sum_{k=0}^n b_k</m>);
        we call <m>\left( b_k \right)</m> the
        <em>sequence of terms</em> of the series.
        <idx><h>series</h></idx>
        The <m>a_n = \sum_{k=1}^n b_k</m>
        (or <m>a_n = \sum_{k=0}^n b_k</m>)
        are the <em>partial sums</em> of the series.
      </p>
    </statement>
  </definition>
  <p>
    If we wanted to be lazy we would define convergence of a series
    simply by referring to convergence of the partial sums of the
    series<mdash/>after all, 
    we just defined series through sequences.
    However, there are some convergence features that take on special
    appearances for series, 
    so we mention them here explicitly.
    For starters, a series <em>converges</em>
    to the <em>limit</em>
    (or <em>sum</em>)
    <m>L</m> by definition if
    <me>
      \lim_{n \to \infty} a_n \ = \ \lim_{n \to \infty} \sum_{k=1}^n b_k
      \ = \ L \, 
    </me>.
    <idx><h>convergent</h><h>series</h></idx>
    <idx><h>limit</h><h>of a series</h></idx>
  </p>
  <p>
    To prove that a series converges we use the definition of limit of
    a sequence: 
    for any <m>\epsilon > 0</m> we have to find an <m>N</m> such that
    for all <m>n \geq N</m>, 
    <me>
      \left| \sum_{k=1}^n b_k - L \right| \ \lt  \ \epsilon \,
    </me>.
    In the case of a convergent series,
    we usually write its limit as
    <m>L = \sum_{k=1}^\infty b_k</m> or <m>L = \sum_{k \geq 1} b_k</m>. 
  </p>
  <example xml:id="ex_geomseries">
    <statement>
      <p>
        Fix <m>z \in \C</m> with <m>|z| \lt  1</m>.
        We claim that the <em>geometric series</em>
        <m>\sum_{ k \ge 1 } z^k</m> converges with limit
        <me>
          \sum_{ k \ge 1 } z^k \ = \ \frac z {1-z} \,
        </me>.
        <idx><h>geometric series</h></idx>
      </p>
      <p>
        In this case, we can compute the partial sums explicitly:
        <me>
          \sum_{k=1}^n z^k \ = \ z + z^2 + \dots + z^n \ = \ \frac{ z -
          z^{n+1} }{ 1 - z } \, 
        </me>,
        whose limit as <m>n \to \infty</m> exists by
        <xref ref="r_n-_0"/>,
        because <m>|z|\lt 1</m>. 
      </p>
    </statement>
  </example>
    <sage>
      <input>
        var('k', 'z')
        assume(abs(z) &lt; 1)
        sum(z^k,k,1, +oo)
      </input>
      <output>
        -z/(z - 1)
      </output>
    </sage>
  <example xml:id="ex_telescope">
    <statement>
      <p>
        Another series whose limit we can compute by manipulating the
        partial sums is 
        <md>
          <mrow>\sum_{k\ge1} \frac1{k^2 + k} \amp \ = \
          \lim_{n\to\infty}\sum_{k=1}^n
          \left(\frac1k-\frac1{k+1}\right)
          </mrow>
          <mrow>\amp \ = \
          \lim_{n\to\infty}\left(1-\frac12+\frac12 -\frac13 
           + \dots + \frac1n-\frac1{n+1}\right)</mrow> 
          <mrow>\amp \ = \ \lim_{n\to\infty}\left(1-\frac1{n+1}\right) \ = \
          1 \, </mrow> 
        </md>.
        A series where most of the terms cancel like this is called
        <em>telescoping</em>.
      </p>
    </statement>
  </example>
    <sage>
      <input>
        var('k')
        sum(1/(k^2+k),k,1, +oo)
      </input>
      <output>
        1
      </output>
    </sage>
  <p>
    Most of the time we can use the completeness property to check
    convergence of a series, 
    and it is fortunate that the Monotone Sequence Property has a
    convenient translation into the language of series of real
    numbers. 
    The partial sums of a series form a nondecreasing sequence if the
    terms of the series are nonnegative, 
    and this observation immediately yields the following:
  </p>
  <corollary xml:id="positiveseries">
    <statement>
      <p>
        If <m>b_k \in \R_{ \ge 0 }</m> then
        <m>\sum_{k \ge 1} b_k</m> converges if and only if the
        partial sums are bounded. 
      </p>
    </statement>
  </corollary>
  <example>
    <statement>
      <p>
        With this new terminology,
        we can revisit <xref ref="ex_e-1series"/>: Let <m>b_k = \frac
        1 {k!}</m>. 
        In <xref ref="ex_e-1series"/>
        we showed that the partial sums
        <me>
          \sum_{ k=1 }^{ n } b_k \ = \ \sum_{ k=1 }^{ n } \frac 1 {k!}
        </me>
        are bounded,
        and <m>\sum_{ k \ge 1 } \frac 1 {k!} = e-1</m>.
      </p>
    </statement>
  </example>
  <p>
    Although <xref ref="positiveseries"/>
    is a mere direct consequence of the completeness property of <m>\R</m>,
    it is surprisingly useful.
    Here is one application, sometimes called the
    <em>Comparison Test</em>:
    <idx><h>comparison test</h></idx>
  </p>
  <corollary xml:id="cor_comparisonseries">
    <statement>
      <p>
        If <m>b_k \ge c_k \ge 0</m> for all <m>k \ge 1</m> and
        <m>\sum_{k \ge 1} b_k</m> converges then so does <m>
        \sum_{k \ge 1} c_k </m>. 
      </p>
    </statement>
    <proof>
      <p>
        By <xref ref="positiveseries"/>,
        the partial sums <m>\sum_{k=1}^n b_k</m> are bounded, and thus so are
        <me>
          \sum_{k=1}^n c_k \ \le \ \sum_{k=1}^n b_k \,
        </me>.
        But this means,
        again by <xref ref="positiveseries"/>,
        that <m>\sum_{k \ge 1} c_k</m> converges.
      </p>
    </proof>
  </corollary>
  <proposition xml:id="generaltermto0">
    <statement>
      <p>
        If <m>\sum_{k \geq 1} b_k</m> converges then <m>\lim_{ n \to \infty } b_n = 0 </m>.
      </p>
    </statement>
  </proposition>
  <p>
    The contrapositive of this proposition is often used,
    sometimes called the <em>Test for Divergence</em>:
  </p>
  <corollary xml:id="cor_divtest">
    <statement>
      <p>
        If <m>\lim_{n \to \infty} b_n \neq 0</m> or <m>\lim_{n
        \to \infty} b_n</m> does not exist, 
        then <m>\sum_{k \geq 1} b_k</m> diverges.
      </p>
    </statement>
  </corollary>
  <example xml:id="ex_geomseriesdiv">
    <statement>
      <p>
        Continuing <xref ref="ex_geomseries"/>,
        for <m>|z| \ge 1</m> the geometric series
        <m>\sum_{ k \ge 1 } z^k</m> diverges since in this case
        <m>\lim_{ n \to \infty } z^n</m> either does not exist or is
        not<nbsp/>0. 
      </p>
    </statement>
    <proof>
      <p>
        Suppose <m>\sum_{k \geq 1} b_k</m> converges.
        Then, using <xref ref="limitrules"/> a) &amp; (d),
        <me>
          0 \ = \ \lim_{n \to \infty} \sum_{ k=1 }^n b_k - \lim_{n \to
          \infty} \sum_{ k=1 }^{ n-1 } b_k \ = \ \lim_{n \to \infty}
          \left( \sum_{ k=1 }^n b_k - \sum_{ k=1 }^{ n-1 } b_k \right)
          \ = \ \lim_{n \to \infty} b_n \,
        </me>.
      </p>
    </proof>
  </example>
  <p>
    A common mistake is to try to use the converse of
    <xref ref="generaltermto0"/>,
    but the converse is false:
  </p>
  <example xml:id="ex_harmonic">
    <statement>
      <p>
        The <em>harmonic series</em> <m>\sum_{k\ge1} \frac 1 k</m>
        diverges 
        (even though the terms go to <m>0</m>):
        If we assume the series converges to <m>L</m>, then
        <md>
          <mrow>L \ \amp = \ 1+\frac12 + \frac13 + \frac 14 + \frac 15
          + \frac 16 + \cdots</mrow> 
          <mrow>\amp > \ \frac 1 2 + \frac 1 2 + \frac 1 4 + \frac 1 4
          + \frac 1 6 + \frac 1 6 + \cdots</mrow> 
          <mrow>\amp = \ 1 + \frac 1 2 + \frac 1 3 + \cdots</mrow> 
          <mrow>\amp = \ L \, </mrow>
        </md>,
        a contradiction. 
      </p>
    </statement>
  </example>
  <proposition xml:id="prop_integraltest">
    <title>Integral Test</title>
    <statement>
      <p>
        If <m>f: [1,\infty) \to \R_{ \ge 0 }</m> is continuous and
        nonincreasing, then 
        <me>
          \int_1^\infty f(t)\,\diff{t} \ \le \ \sum_{k \ge 1} f(k) \
          \le \ f(1) + \int_1^\infty f(t)\,\diff{t} \, 
        </me>.
        <idx><h>integral test</h></idx>
      </p>
    </statement>
  </proposition>
  <p>
    The Integral Test literally comes with a proof by
    picture<mdash/>see <xref ref="fig_integraltest"/>:
    the integral of <m>f</m> on the interval <m>[k,k+1]</m> is bounded
    between <m>f(k)</m> and <m>f(k+1)</m>. 
    Adding the pieces gives the inequalities above for the <m>n</m>th
    partial sum versus the integrals from <m>1</m> to <m>n</m> and
    from <m>1</m> to <m>n+1</m>, 
    and the inequality persists in the limit.
  </p>
  <figure xml:id="fig_integraltest">
    <caption>The integral test.</caption>
    <sidebyside widths="45% 45%">
      <image>
        <prefigure xmlns="https://prefigure.org"
                   label="integral-test-a">
          <xi:include href="prefigure/integral-test-a.xml"/>
        </prefigure>
      </image>
      <image>
        <prefigure xmlns="https://prefigure.org"
                   label="integral-test-b">
          <xi:include href="prefigure/integral-test-b.xml"/>
        </prefigure>
      </image>
    </sidebyside>
  </figure>
  <corollary xml:id="cor_integraltest">
    <statement>
      <p>
        If <m>f: [1,\infty) \to \R_{ \ge 0 }</m> is continuous and
        nonincreasing, 
        then <m>\sum_{k \ge 1} f(k)</m> converges if and only if
        <m>\int_1^\infty f(t)\,\diff{t}</m> is finite. 
      </p>
    </statement>
  </corollary>
  <proof>
    <p>
      Suppose <m>\int_1^\infty f(t)\,\diff{t} = \infty</m>.
      Then the first inequality in <xref ref="prop_integraltest"/>
      implies that the partial sums <m>\sum_{k=1}^n f(k)</m> are unbounded,
      and so <xref ref="positiveseries"/>
      says that <m>\sum_{k \ge 1} f(k)</m> cannot converge.
    </p>
    <p>
      Conversely, if <m>\int_1^\infty f(t)\,\diff{t}</m> is finite
      then the second inequality in <xref ref="prop_integraltest"/> 
      says that the partial sums <m>\sum_{k=1}^n f(k)</m> are bounded;
      thus, again with <xref ref="positiveseries"/>,
      we conclude that <m>\sum_{k \ge 1} f(k)</m> converges.
    </p>
  </proof>
  <example xml:id="exam_riemannzetaprep">
    <statement>
      <p>
        The series <m>\sum_{k\ge1} \frac 1 {k^p}</m> converges for
        <m>p > 1</m> and diverges for <m>p \lt  1</m> 
        (and the case <m>p=1</m> was the subject of <xref ref="ex_harmonic"/>)
        because
        <me>
          \int_1^\infty \frac{ \diff{x} }{ x^p } \ = \ \lim_{ a \to
          \infty } \frac{ a^{ -p+1 } }{ -p+1 } + \frac 1 { p-1 } 
        </me>
        is finite if and only if <m>p > 1</m>. 
      </p>
    </statement>
  </example>
  <p>
    By now you might be amused that we have collected several results
    on series whose terms are nonnegative real numbers. 
    One reason is that such series are a bit easier to handle,
    another one is that there is a notion of convergence special to
    series that relates any series to one with only nonnegative terms: 
  </p>
  <definition>
    <statement>
      <p>
        The series <m>\sum_{k \geq 1} b_k</m>
        <em>converges absolutely</em>
        if <m>\sum_{k \geq 1} \left| b_k \right|</m> converges.
        <idx><h>absolute convergence</h></idx>
      </p>
    </statement>
  </definition>
  <theorem xml:id="absconvthm">
    <statement>
      <p>
        If a series converges absolutely then it converges.
      </p>
    </statement>
  </theorem>
  <p>
    This seems like an obvious statement,
    but its proof is, nevertheless, nontrivial.
  </p>
  <proof>
    <p>
      Suppose <m>\sum_{k \geq 1} \left| b_k \right|</m> converges.
      We first consider the case that each <m>b_k</m> is real.
      Let
      <me>
        b_k^+ := \begin{cases}b_k \amp  \text{ if }  b_k \ge 0, \\ 0
        \amp  \text{ otherwise } \end{cases} \qquad \text{ and }
        \qquad b_k^- := \begin{cases}b_k \amp  \text{ if }  b_k \lt
        0, \\ 0   \amp  \text{ otherwise. } \end{cases} 
      </me>
      Then <m>0 \le b_k^+ \le |b_k|</m> and
      <m>0 \le - b_k^- \le |b_k|</m> for all <m>k \ge 1</m>,
      and so by <xref ref="cor_comparisonseries"/>, both
      <me>
        \sum_{ k \ge 1 } b_k^+ \qquad \text{ and }  \qquad - \sum_{ k
        \ge 1 } b_k^- 
      </me>
      converge.
      But then so does
      <me>
        \sum_{ k \ge 1 } b_k \ = \ \sum_{ k \ge 1 } b_k^+ + \sum_{ k \ge
        1 } b_k^- 
      </me>.
    </p>
    <p>
      For the general case <m>b_k \in \C</m>,
      we write each term as <m>b_k = c_k + i \, d_k</m>.
      Since <m>0 \le |c_k| \le |b_k|</m> for all <m>k \ge 1</m>,
      <xref ref="cor_comparisonseries"/>
      implies that <m>\sum_{ k \ge 1 } c_k</m> converges absolutely,
      and by an analogous argument,
      so does <m>\sum_{ k \ge 1 } d_k</m>.
      But now we can use the first case to deduce that both <m>\sum_{
      k \ge 1 } c_k</m> and 
      <m>\sum_{ k \ge 1 } d_k</m> converge, and thus so does
      <me>
        \sum_{ k \ge 1 } b_k \ = \ \sum_{ k \ge 1 } c_k + i \sum_{ k \ge
        1 } d_k \, 
      </me>.
    </p>
  </proof>
  <example xml:id="exam_riemannzet">
    <statement>
      <p>
        Continuing <xref ref="exam_riemannzetaprep"/>,
        <me>
          \zeta(z) \ := \ \sum_{k\ge1} \frac 1 {k^z}
        </me>
        converges for <m>\Re(z)>1</m>,
        because then (using <xref ref="ex_absolutepowers"/>)
        <me>
          \sum_{k\ge1} \left| k^{ -z } \right| \ = \ \sum_{k\ge1} k^{ - \Re(z) }
        </me>
        converges.
        Viewed as a function in <m>z</m>,
        the series <m>\zeta(z)</m> is the
        <em>Riemann zeta function</em>,
        an indispensable tool in number theory and many other
        <idx><h>Riemann zeta function</h></idx>
        areas in mathematics and physics.<fn xml:id="riemannzeta">
        The Riemann zeta function is the subject of the arguably most
        famous open problem in mathematics, 
        the <em>Riemann hypothesis</em>.
        It turns out that <m>\zeta(z)</m> can be extended to a
        function that is holomorphic on <m>\C \setminus \{ 1 \}</m>, 
        and the Riemann hypothesis asserts that the roots of this
        extended function in the strip 
        <m>0 \lt  \Re(z) \lt  1</m> are all on the <em>critical
        line</em> 
        <m>\Re(z) = \frac 1 2</m>.
        </fn> 
      </p>
    </statement>
  </example>
  <p>
    Another common mistake is to try to use the converse of
    <xref ref="absconvthm"/>,
    which is also false:
  </p>
  <example xml:id="ex_altharmonic">
    <statement>
      <p>
        The <em>alternating harmonic series</em>
        <m>\sum_{k\ge1}\frac{(-1)^{k+1}}k</m> converges:
        <md>
          <mrow>\sum_{k\ge1}\frac{(-1)^{k+1}}k \amp \ = \ 1-\frac12 +
          \frac13 - \frac 14 + \frac15 - \frac16 +  \cdots</mrow> 
          <mrow>\amp \ = \ \left(1-\frac12\right) +
          \left(\frac13-\frac14\right) + \left(\frac15-\frac16\right)
          + \cdots</mrow> 
        </md>
        <idx><h>alternating harmonic series</h></idx> 
        (There is a small technical detail to be checked here,
        since we are effectively ignoring half the partial sums of the
        original series; 
        see <xref ref="ex_groupingterms"/>.) Since
        <me>
          \frac1{2k-1}-\frac1{2k} \ = \ \frac1{2k(2k-1)} \ \le \ \frac 1
          { (2k-1)^2 } \ \le \ \frac 1 { k^2 } \, 
        </me>,
        <m>\sum_{k\ge1}\frac{(-1)^{k+1}}k</m> converges by
        <xref ref="cor_comparisonseries"/>
        and <xref ref="exam_riemannzetaprep"/>.
      </p>
      <p>
        However, according to <xref ref="ex_harmonic"/>,
        <m>\sum_{k\ge1}\frac{(-1)^{k+1}}k</m> does <em>not</em>
        converge absolutely.
      </p>
    </statement>
  </example>
    <sage>
      <input>
        var('k')
        sum((-1)^k/k,k,1, +oo)
      </input>
      <output>
        -log(2)
      </output>
    </sage>
</section>
