<?xml version="1.0" encoding="UTF-8"?>
<section xmlns:xi="http://www.w3.org/2001/XInclude"
         xml:id="sec_geometricprops">
  <title>Geometric Properties</title>
  <p>
    From the chain of basic inequalities
    <me>- \sqrt{ x^2 + y^2 } \le - \sqrt{ x^2 } \le x \le \sqrt{ x^2 }
    \le \sqrt{ x^2 + y^2 }
    </me> (or,
    alternatively,
    by arguing with basic geometric properties of triangles),
    we obtain the inequalities
    <men xml:id="trianglegeom">
      -|z| \ \leq \ \Re(z) \ \leq \ |z| \qquad \text{ and }  \qquad
      -|z| \ \leq \ \Im(z) \ \leq \ |z| \, 
    </men>.
  </p>
  <p>
    The square of the absolute value has the nice property
    <me>
      \left| x+iy \right|^2 \ = \ x^2 + y^2 \ = \ (x+iy) (x-iy) \,
    </me>.
  </p>
  <p>
    This is one of many reasons to give the process of passing from
    <m>x+iy</m> to <m>x-iy</m> a special name. 
  </p>
  <definition>
    <statement>
      <p>
        The number <m>x-iy</m> is the <em>(complex) conjugate</em>
        of <m>x+iy</m>.
        <idx><h>conjugate</h></idx>
        We denote the conjugate by
        <me>
          \overline{x+iy} \ := \ x-iy \,
        </me>.
      </p>
    </statement>
  </definition>
  <p>
    Geometrically,
    conjugating <m>z</m> means reflecting the vector corresponding to
    <m>z</m> with respect to the real axis, as shown in <xref
    ref="fig-conjugate"/>.
  </p>

  <figure xml:id="fig-conjugate">
    <image width="50%">
      <prefigure xmlns="https://prefigure.org"
                 label="conjugate-def">
        <xi:include href="prefigure/conjugate.xml"/>
      </prefigure>
    </image>
    <caption>
      The complex conjugate <m>\conj{z}</m> is
      obtained by reflecting <m>z</m> across the real axis.
    </caption>
  </figure>

  <p>
    The following proposition collects some basic properties of the
    conjugate. 
  </p>
  <proposition xml:id="conjugation">
    <statement>
      <p>
        For any <m>z, z_1, z_2 \in \C</m>, 
        <ol marker="(a) ">
          <li>
            <p>
              <m>\conj{z_1 \pm z_2} = \conj{z_1}\pm\conj{z_2}</m>
            </p>
          </li>
          <li xml:id="conjugationmult">
            <p>
              <m>\conj{z_1 \cdot z_2} = \conj{z_1}\cdot\conj{z_2}</m>
            </p>
          </li>
          <li>
            <p>
              <m>\conj{ \left( \frac{ z_1 }{ z_2 } \right) } = \frac{
              \ \conj{z_1} \ }{ \conj{z_2} }</m> 
            </p>
          </li>
          <li>
            <p>
              <m>\conj{\, \conj{z} \, }=z</m>
            </p>
          </li>
          <li>
            <p>
              <m>\abs{\conj{z}}=\abs z</m>
            </p>
          </li>
          <li xml:id="i_zzbar">
            <p>
              <m>\abs{z}^2=z\conj z</m>
            </p>
          </li>
          <li>
            <p>
              <m>\Re(z) = \frac 1 2 \left( z+\conj z \right)</m>
            </p>
          </li>
          <li>
            <p>
              <m>\Im(z) = \frac{ 1 }{ 2i } \left( z-\conj z \right)</m>
            </p>
          </li>
          <li>
            <p>
              <m>\conj{e^{i\phi}}=e^{-i\phi}</m>.
            </p>
          </li>
        </ol>
      </p>
    </statement>
  </proposition>
  <p>
    The proofs of these properties are straightforward (see <xref
    ref="ex_conjugation"/>);
    once more we give a sample (b).
  </p>
  <proof>
    <p>
      Let <m>z_1 = x_1 + i y_1</m> and <m>z_2 = x_2 + i y_2</m>.
      Then
      <md>
        <mrow>\conj{z_1 \cdot z_2} \amp \ = \ \conj{ (x_1 x_2 - y_1 y_2)
        + i ( x_1 y_2 + x_2 y_1 ) }
        </mrow>
        <mrow>
          \amp \ = \ (x_1 x_2 - y_1 y_2) - i ( x_1 y_2 + x_2 y_1 )
        </mrow>
        <mrow>
          \amp \ = \ (x_1 - i y_1) (x_2 - i y_2)
        </mrow>
        <mrow>
          \amp \ = \ \conj{z_1}\cdot\conj{z_2} \, .
        </mrow>
      </md>
    </p>
  </proof>
  <p>
    We note that the property
    <m>\abs{z}^2=z\conj z</m>
    yields a neat formula for the inverse of a nonzero complex number,
    which is implicit already in <xref ref="eq-lastmult"/>:
    <me>
      z^{-1} \ = \ \frac1z \ = \ \frac{\conj z}{\abs{z}^2} \,
    </me>.
  </p>
  <p>
    A famous geometric inequality
    (which holds, more generally,
    for vectors in <m>\R^n</m>)
    goes as follows.
  </p>
  <proposition xml:id="lem_triangleineq">
    <title>Triangle inequality</title>
    <statement>
      <p>
            <idx><h>triangle inequality</h></idx>
        For any <m>z_1, z_2 \in \C</m> we have <m>\ds \left| z_1 + z_2 \right| \leq \left| z_1 \right| + \left| z_2 \right| </m>.
      </p>
    </statement>
  </proposition>
  <p>
    By drawing a picture in the complex plane,
    you should be able to come up with a geometric proof of the
    triangle inequality. 
    Here we proceed algebraically:
  </p>
  <proof>
    <p>
      We make extensive use of <xref ref="conjugation"/>:
      <md>
        <mrow>
          \left| z_1 + z_2 \right|^2 \amp = \ \left( z_1 + z_2
          \right) \o{ \left( z_1 + z_2 \right) }
        </mrow>
        <mrow>
          \amp \ = \ \left( z_1 + z_2
          \right) \left( \o{z_1} + \o{z_2} \right)
        </mrow>
        <mrow>
          \amp \ = \ z_1 \o{z_1} + z_1
          \o{z_2} + z_2 \o{z_1} + z_2 \o{z_2}
        </mrow> 
        <mrow>
          \amp = \ \left| z_1 \right|^2 + z_1 \o{z_2} + \o{ z_1 \o{z_2}
          } + \left| z_2 \right|^2
        </mrow>
        <mrow>
          \amp \ = \ \left| z_1 \right|^2 + 2 \Re
          \left( z_1 \o{z_2} \right) + \left| z_2 \right|^2
        </mrow>
        <mrow>
          \amp \leq \ \left| z_1 \right|^2 + 2 \left| z_1 \o{z_2}
          \right| + \left| z_2 \right|^2
        </mrow>
        <mrow>
          \amp \ = \ \left| z_1 \right|^2 + 2
          \left| z_1 \right| \left| \o{z_2} \right| + \left| z_2
          \right|^2
        </mrow>
        <mrow>
          \amp \ = \ \left| z_1 \right|^2 + 2 \left| z_1 \right|
          \left| z_2 \right| + \left| z_2 \right|^2
        </mrow>
        <mrow>
          \amp = \ \left( \left| z_1 \right| + \left| z_2 \right|
          \right)^2
        </mrow>
      </md>,
      where the inequality follows from <xref ref="trianglegeom"/>.
      Taking square roots on the left- and right-hand sides proves our
      claim. 
    </p>
  </proof>
  <p>
    For future reference we list several useful variants of the
    triangle inequality: 
  </p>
  <corollary xml:id="cor_triangleineq">
    <statement>
      <p>
        For <m>z_1, z_2, \dots, z_n \in \C</m>,
        we have the following relations:
        <ol marker="(a) ">
          <li xml:id="trianineqcor">
            <p>
              The triangle inequality:
              <me>
                \abs{\pm z_1\pm z_2} \le
                \abs{z_1}+\abs{z_2}
              </me>.
            </p>
          </li>
          <li xml:id="revtrianineq">
            <p>
              The reverse triangle inequality:
              <me>
                \abs{\pm z_1\pm z_2} \ge \bigl|
                \abs{z_1}-\abs{z_2} \bigr| <nbsp/>
              </me>.
              <idx><h>reverse triangle inequality</h></idx>
              <idx><h>triangle inequality</h><h>reverse</h></idx> 
            </p>
          </li>
          <li xml:id="trianineqsum">
            <p>
              The triangle inequality for sums:
              <me>
                \abs{\sum_{k=1}^n z_k} \ \le \ \sum_{k=1}^n \abs{z_k} 
              </me>.
            </p>
          </li>
        </ol>
      </p>
    </statement>
  </corollary>
  <p>
    <xref ref="trianineqcor"/>
    is just a rewrite of the original triangle inequality,
    using the fact that <m>\abs{\pm z}=\abs{z}</m>,
    and <xref ref="trianineqsum"/> follows by induction.
    The proof of the reverse triangle inequality
    is left as <xref ref="ex_reversetriangle"/>.
  </p>
</section>
