<section xml:id="sec_residues">
  <title>Residues</title>
  <p>
    We now pick up the thread from <xref ref="cor_firstresidue">Corollary</xref>
    and apply it to the Laurent series
    <me>
      f(z) \= \sz c_k \left( z - z_0 \right)^k
    </me>
    at an isolated singularity <m>z_0</m> of <m>f</m>.
    It says that if <m>\gg</m> is any positively oriented,
    simple, closed,
    piecewise smooth path in the punctured disk of convergence of this Laurent series,
    and <m>z_0</m> is inside<nbsp/><m>\gg</m>, then
    <me>
      \int_\gg f(z) \, \diff{z} \= 2 \pi i \, c_{ -1 } \,
    </me>.
  </p>
  <definition>
    <statement>
      <p>
        Suppose <m>z_0</m> is an isolated singularity of <m>f</m> with Laurent series <m>\sz c_k (z - z_0)^k</m>.
        Then <m>c_{-1}</m> is the <em>residue
            <idx><h>residue</h></idx>
        of <m>f</m> at <m>z_0</m></em>,
        denoted by <m>\Res_{z=z_0} (f(z))</m> or <m>\Res (f(z) , \, z=z_0)</m>.
      </p>
    </statement>
  </definition>
  <p>
    <xref ref="cor_firstresidue">Corollary</xref>
    suggests that we can compute integrals over closed curves by finding the residues at isolated singularities,
    and our next theorem makes this precise.
  </p>
  <theorem xml:id="residuethm">
    <title>Residue Theorem</title>
    <statement>
      <p>
            <idx><h>residue theorem</h></idx>
        Suppose <m>f</m> is holomorphic in the region <m>G</m>, except for isolated singularities, and <m>\gg</m> is a positively oriented, simple, closed, piecewise smooth path that avoids the singularities of <m>f</m>, and <m>\gg \sim_G 0</m>.
        Then there are only finitely many singularities inside <m>\gg</m>, and
        <me>
          \int_\gg f \= 2 \pi i \, \sum_k \Res_{z=z_k} (f(z))
        </me>
        where the sum is taken over all singularities <m>z_k</m> inside <m>\gg</m>.
      </p>
    </statement>
  </theorem>
  <figure xml:id="residuethmpic">
    <caption>Proof of <xref ref="residuethm">Theorem</xref>.</caption>
    <image source="images/picturec1a8d91a6a_rev.png"/>
  </figure>
  <proof>
    <p>
      First, let <m>S</m> be the set of singularities inside <m>\gg</m>.
      The set <m>S</m> is closed
      (since the points in <m>G</m> where <m>f</m> is holomorphic form an open set)
      and bounded
      (since the inside of <m>\gg</m> is bounded),
      and the points of <m>S</m> are isolated in <m>S</m>
      (by <xref ref="classificationzeros">Theorem</xref>
      <xref ref="classificationzeros_isolated"></xref>).
      An application of <xref ref="ex_compactAndIsolated">Exercise</xref>
      shows that <m>S</m> is finite.
    </p>
    <p>
      Now we follow the approach started in <xref ref="fig_laurentmotivation">Figure</xref>:
      as with that integration path, we
      <q>subdivide</q>
      <m>\gg</m> so that we can replace it by closed curves around the singularities inside <m>\gg</m>.
      These curves, in turn,
      can then be transformed to circles around the singularities,
      as suggested by <xref ref="residuethmpic">Figure</xref>.
      By Cauchy's <xref ref="cauchythm">Theorem</xref>,
      <m>\int_\gg f</m> equals the sum of the integrals of <m>f</m> over these circles.
      Now use <xref ref="cor_firstresidue">Corollary</xref>.
    </p>
  </proof>
  <p>
    Computing integrals is as easy
    (or hard!)
    as computing residues.
    The following two propositions start the range of tricks you may use when computing residues.
  </p>
  <proposition xml:id="prop_residueAsLimit">
    <statement>
      <p>
        \hangindent\leftmargini \mbox{(a)} If <m>z_0</m> is a removable singularity of <m>f</m> then <m>\ds \Res_{z=z_0}(f(z)) = 0</m>.
        <ol marker="a">
          <li>
            <p>
              If <m>z_0</m> is a pole of <m>f</m> of order <m>n</m> then
              <me>
                \Res_{z=z_0} (f(z)) \= \frac 1 {(n-1)!} \lim_{z \to z_0} \frac{ d^{n-1} }{ \diff{z}^{n-1} } \bigl( (z - z_0)^n f(z) \bigr) \,
              </me>.
            </p>
          </li>
        </ol>
      </p>
    </statement>
  </proposition>
  <proof>
    <p>
      (a) follows from <xref ref="singlaurent">Proposition</xref>(a).
    </p>
    <p>
      (b) We know by <xref ref="singlaurent">Proposition</xref>(b) that the Laurent series at <m>z_0</m> looks like
      <me>
        f(z) = \sum_{k \geq -n} c_k (z-z_0)^k
      </me>.
    </p>
    <p>
      But then
      <me>
        (z - z_0)^n f(z) = \sum_{k \geq -n} c_k (z-z_0)^{k+n}
      </me>
      is a power series, and we can use Taylor's formula
      (<xref ref="taylor">Corollary</xref>)
      to compute <m>c_{-1}</m>.
    </p>
  </proof>
  <p>
    It is worth noting that we are really coming full circle here:
    compare this proposition to Cauchy's Integral Formulas
    (<xref ref="cauchyformula">Theorems</xref> &amp;
    <xref ref="cauchyformula2"></xref>
    and <xref ref="cauchyformula3">Corollary</xref>).
  </p>
  <example xml:id="ex_expoversinrev">
    <statement>
      <p>
        The integrand <m>\frac{ \exp(z) }{ \sin(z) }</m> in <xref ref="ex_expoversin">Example</xref>
        has poles of order 1 at 0 and <m>\pi</m>.
        We thus compute
        <me>
          \Res_{ z=0 } \left( \frac{ \exp(z) }{ \sin(z) } \right) \= \lim_{ z \to 0 } \left( z \, \frac{ \exp(z) }{ \sin(z) } \right) \= \exp(0) \lim_{ z \to 0 } \frac{ z }{ \sin(z) } \= 1
        </me>
        and
        <me>
          \Res_{ z=\pi } \left( \frac{ \exp(z) }{ \sin(z) } \right) \= \lim_{ z \to \pi } \left( (z-\pi) \, \frac{ \exp(z) }{ \sin(z) } \right) \= \exp(\pi) \lim_{ z \to \pi } \frac{ z-\pi }{ \sin(z) } \= - e^\pi
        </me>,
        confirming our computations in <xref ref="ex_expoversin">Example</xref>. \pushQED{}\popQED
      </p>
    </statement>
  </example>
  <example>
    <statement>
      <p>
        Revisiting <xref ref="ex_sinoverz3">Example</xref>,
        the function <m>f(z) = \frac{ \sin(z) }{ z^3 }</m> has a double pole at 0 with
        <me>
          \Res_{ z=0 } \left( \frac{ \sin(z) }{ z^3 } \right) \= \lim_{ z \to 0 } \frac{ d }{ \diff{z} } \left( z^2 \, \frac{ \sin(z) }{ z^3 } \right) \= \lim_{ z \to 0 } \left( \frac{ z \cos(z) -  \sin(z) }{ z^2 } \right) \= 0 \,
        </me>,
        after a few iterations of L'H&#xf4;pital's Rule.
        (In this case,
        it is simpler to read the residue off the Laurent series in <xref ref="ex_sinoverz3">Example</xref>.)
        \pushQED{}\popQED
      </p>
    </statement>
  </example>
  <proposition xml:id="lem_computing_residues2">
    <statement>
      <p>
        Suppose <m>f</m> and <m>g</m> are holomorphic at <m>z_0</m>,
        which is a simple zero of <m>g</m> (i.e., a zero of multiplicity 1).
        Then
        <me>
          \Res_{z=z_0} \left( \frac{ f(z) }{ g(z) } \right) \= \frac{ f(z_0) }{ g'(z_0) } \,
        </me>.
      </p>
    </statement>
  </proposition>
  <proof>
    <p>
      The functions <m>f</m> and <m>g</m> have power series centered at <m>z_0</m>;
      the one for <m>g</m> has by assumption no constant term:
      <md>
        <mrow>f(z) \amp \= \sum_{k \ge 0} a_k (z-z_0)^k</mrow>
        <mrow>g(z) \amp \= \sum_{k \ge 1} b_k (z-z_0)^k \= (z-z_0) \sum_{k \geq 1} b_k (z-z_0)^{k-1} </mrow>
      </md>.
    </p>
    <p>
      Let <m>\ds h(z) := \sum_{k \geq 1} b_k (z-z_0)^{k-1}</m> and note that <m>h(z_0) = b_1 \ne 0</m>.
      Hence
      <me>
        \frac{ f(z) }{ g(z) } \= \frac{ f(z) }{ (z-z_0) \, h(z) } \,
      </me>,
      and the function <m>\frac f h</m> is holomorphic at <m>z_0</m>.
      By <xref ref="prop_residueAsLimit">Prop</xref>
      and Taylor's formula (<xref ref="taylor">Corollary</xref>),
      <me>
        \Res_{z=z_0} \left( \frac{ f(z) }{ g(z) } \right) \= \lim_{z\to z_0}\left( (z-z_0) \frac{f(z)}{(z-z_0)h(z)}\right) \= \frac{ f(z_0) }{ h(z_0) } \= \frac{ a_0 }{ b_1 } \= \frac{ f(z_0) }{ g'(z_0) } \, . \qedhere
      </me>
    </p>
  </proof>
  <example>
    <statement>
      <p>
        Revisiting once more <xref ref="ex_expoversin">Example</xref>,
        we note that <m>f(z) = \exp(z)</m> and <m>g(z) = \sin(z)</m> fit the bill.
        Thus
        <me>
          \Res_{ z=0 } \left( \frac{ \exp(z) }{ \sin(z) } \right) \= \frac{ \exp(0) }{ \cos(0) } \= 1
        </me>
        and
        <me>
          \Res_{ z=\pi } \left( \frac{ \exp(z) }{ \sin(z) } \right) \= \frac{ \exp(\pi) }{ \cos(\pi) } \= - e^\pi
        </me>,
        confirming once more our computations in <xref ref="ex_expoversin">Examples</xref>
        and <xref ref="ex_expoversinrev"></xref>. \pushQED{}\popQED
      </p>
    </statement>
  </example>
  <example>
    <statement>
      <p>
        We compute the residue of <m>\frac{ z^2 + 2 }{ (\exp(z) - 1) \cos(z) }</m> at <m>z_0 = 2 \pi i</m>,
        by applying <xref ref="lem_computing_residues2">Proposition</xref>
        with <m>f(z) = \frac{ z^2 + 2 }{ \cos(z) }</m> and <m>g(z) = \exp(z) - 1</m>.
        Thus
        <me>
          \Res_{ z = 2 \pi i } \left( \frac{ z^2 + 2 }{ (\exp(z) - 1) \cos(z) } \right) \= \frac{ \frac{ (2 \pi i)^2 + 2 }{ \cos(2 \pi i) } }{ \exp(2 \pi i) } \= \frac{ -4 \pi^2 + 2 }{ \cosh(2 \pi) } \,
        </me>.
      </p>
    </statement>
  </example>
  <p>
    An extension of <xref ref="lem_computing_residues2">Proposition</xref>
    of sorts is given in <xref ref="ex_computing_residues2">Exercise</xref>.
  </p>
</section>