<?xml version="1.0" encoding="utf-8"?>

<section xml:id="sec_Cauchy-Riemann">
  <title>The Cauchy<ndash/>Riemann Equations</title>
  <p>
    When considering a real-valued function <m>f: \R^2 \to \R</m> of
    two variables, 
    there is no notion of <em>the</em>
    derivative of a function.
    For such a function, we instead only have partial derivatives
    <m>\fderiv fx(x_0,y_0)</m> and <m>\fderiv fy(x_0,y_0)</m>
    (and also directional derivatives)
    which depend on the way in which we approach a point <m>(x_0,y_0)
    \in \R^2</m>.
  </p>
  <p>
    For a complex-valued function <m>f(z)</m>,
    we now have a new concept of the derivative <m>f'(z_0)</m>,
    which by definition cannot depend on the way in which we approach
    a point <m>z_0 = (x_0,y_0) \in \C</m>. 
    It is logical, then,
    that there should be a relationship between the complex derivative
    <m>f'(z_0)</m> and the <em>partial derivatives</em>
    <md>
      <mrow>
      \fderiv fx(z_0) \amp := \lim_{ x \to x_0 } \frac{ f(x,y_0) -
      f(x_0,y_0) }{ x - x_0 }
      </mrow>
      <mrow>
      \fderiv fy(z_0) \amp := \lim_{ y \to y_0 } \frac{ f(x_0,y) -
      f(x_0,y_0) }{ y - y_0 } \, 
      </mrow>
    </md>.
    <idx><h>partial derivative</h></idx>
    <idx><h>derivative</h><h>partial</h></idx>
    (so this definition is exactly as in the real-valued case).
  </p>
  <p>
    This relationship between the complex derivative and partial
    derivatives is very strong, 
    and it is a powerful computational tool.
    It is described by the <em>Cauchy<ndash/>Riemann equations</em>,
    named after Augustin Louis Cauchy (1789<ndash/>1857) and Georg
    Friedrich Bernhard Riemann (1826<ndash/>1866), 
    even though the equations appeared already in the works of Jean le
    Rond d'Alembert (1717<ndash/>1783) and Leonhard Euler
    (1707<ndash/>1783). 
    <idx><h>Cauchy<ndash/>Riemann equations</h></idx> 
  </p>

  <theorem xml:id="cre">
    <statement>
      <p>
        <ol marker="(a) ">
          <li>
            <p>Suppose <m>f</m> is differentiable at <m>z_0 = x_0 + i
            y_0</m>. 
            Then the partial derivatives of <m>f</m> exist and satisfy
            <men xml:id="complexcr">
              \fderiv fx(z_0) \ = \ -i \, \fderiv fy(z_0) \,
            </men>
            and the derivative is given by
            <me>
              f'(z_0) \ = \ \fderiv fx(z_0) \,
              </me>.
            </p>
          </li>
          <li>
            <p>Suppose <m>f</m> is a complex function such that the
            partial derivatives <m>\fderiv fx</m> and 
            <m>\fderiv fy</m> exist in an open disk centered at <m>z_0</m>
            and are continuous at <m>z_0</m>. 
            If these partial derivatives satisfy {<xref ref="complexcr"/>}
            then <m>f</m> is differentiable at<nbsp/><m>z_0</m>.
            </p>
          </li>
        </ol>
      </p>
    </statement>
  </theorem>

  <p>
    Before proving <xref ref="cre"/>, we note several comments and
    give two applications.  It is traditional, and often convenient,
    to write the function <m>f</m> in terms of its real and imaginary
    parts.  That is, we write <m>f(z) = f(x,y) = u(x,y) + i \,
    v(x,y)</m> where <m>u</m> is the real part of <m>f</m> and
    <m>v</m> is the imaginary part.  Then, using the usual shorthand
    <m>f_x = \fderiv fx</m> and <m>f_y = \fderiv fy</m>, we have 
    <md>
      <mrow>
        f_x \amp \ = \ u_x+i \, v_x
      </mrow>
      <mrow>
        -if_y \amp \ = \ -i(u_y+i \, v_y) \ = \ v_y-i \, u_y \,
      </mrow>
    </md>.
  </p>
  <p>
    With this terminology we can rewrite <xref ref="complexcr"/> as
    the pair of equations 
    <men xml:id="crequations">
      \begin{array}{ccc}
        u_x(x_0,y_0) \amp  = \amp v_y(x_0,y_0) \\
        u_y(x_0,y_0) \amp  = \amp -v_x(x_0,y_0) \, .
      \end{array}
    </men>
  </p>
  <p>
    As stated, parts (a) and (b) in <xref ref="cre"/>
    are not quite converse statements.
    However, we will show in <xref ref="infdiff"/>
    that if <m>f</m> is <em>holomorphic</em>
    at <m>z_0 = x_0 + i y_0</m> then <m>u</m> and <m>v</m> have
    continuous partials 
    (of any order)
    at <m>z_0</m>.
    That is, in <xref ref="cachyconschapter"/>
    we will see that <m>f = u + i v</m> is holomorphic in an open set
    <m>G</m> if and only if <m>u</m> and <m>v</m> have continuous
    partials that satisfy <xref ref="crequations"/>
    in<nbsp/><m>G</m>. 
  </p>
  <p>
    If <m>u</m> and <m>v</m> satisfy <xref ref="crequations"/> and
    their second partials are also continuous, then 
    <men xml:id="eq_firstharmonicinstance">
      u_{xx}(x_0,y_0) \ = \ v_{yx}(x_0,y_0) \ = \ v_{xy}(x_0,y_0) \ = \ - u_{yy}(x_0,y_0) \,
    </men>,
    that is,
    <me>
      u_{xx}(x_0,y_0) + u_{yy}(x_0,y_0) \ = \ 0
    </me>
  </p>
  <p>
    (and an analogous identity for <m>v</m>).
    Functions with continuous second partials satisfying this partial
    differential equation on a region <m>G \subset \C</m> 
    (though not necessarily <xref ref="crequations"/>)
    are called <em>harmonic</em>
    on <m>G</m>;
    we will study such functions in <xref ref="harmonicChapter"/>.
    <idx><h>harmonic</h></idx>
    Again, as we will see later,
    if <m>f</m> is holomorphic in an open set <m>G</m> then the
    partials of any order of <m>u</m> and <m>v</m> exist; 
    hence we will show that the real and imaginary parts of a function
    that is holomorphic in an open set are harmonic on that set. 
  </p>
  <example>
    <statement>
      <p>
        We revisit <xref ref="exam_zcubedentire">Example</xref>
        and again consider <m>f: \C \to \C</m> given by
        <me>
          f(z) \ = \ z^3 \ = \ (x+iy)^3 \ = \ \left( x^3 - 3xy^2 \right) + i
          \left( 3 x^2 y - y^3 \right) \,
        </me>.
      </p>
      <p>
        Thus
        <me>
          f_x(z) \ = \ 3x^2 - 3y^2 + 6i xy \quad \text{ and } \quad
          f_y(z) \ = \ -6 xy + 3i x^2 - 3i y^2 
        </me>
        are continuous on <m>\C</m> and satisfy <m>f_x = -i f_y</m>.
        Thus by <xref ref="cre">Theorem</xref>(b),
        <m>f(z) = z^3</m> is entire. 
      </p>
    </statement>
  </example>
  <example>
    <statement>
      <p>
        Revisiting <xref ref="exam_zbarsquareddiff">Example</xref>
        (you saw that coming, didn't you?),
        we consider <m>f: \C \to \C</m> given by
        <me>
          f(z) \ = \ (\conj z)^2 \ = \ (x-iy)^2 \ = \ x^2 - y^2 - 2ixy \,
        </me>.
      </p>
      <p>
        Now
        <me>
          f_x(z) \ = \ 2x - 2iy \qquad \text{ and }  \qquad f_y(z) \ = \ -2y - 2ix \,
        </me>,
        which satisfy <m>f_x = -i f_y</m> only when <m>z=0</m>. (The
        contrapositive of) <xref ref="cre"/>(a) thus
        implies that 
        <m>f(z) = (\conj z)^2</m> is not differentiable on <m>\C
        \setminus \{ 0 \}</m>.
      </p>
    </statement>
  </example>
  <proof>
    <p>
      (a) If <m>f</m> is differentiable at <m>z_0 = (x_0, y_0)</m> then
      <me>
        f'(z_0) \ = \ \lim_{\D z \to 0}\frac{f(z_0+\D z) - f(z_0)}{\D z} \,
      </me>.
    </p>
    <p>
      As we know by now,
      we must get the same result if we restrict <m>\D z</m> to be on
      the real axis and if we restrict it to be on the imaginary
      axis. 
      In the first case, <m>\D z=\D x</m> and
      <md>
        <mrow>
        f'(z_0) \amp \ = \ \lim_{\D x \to 0}\frac{f(z_0+\D x) -
        f(z_0)}{\D x}
        </mrow>
        <mrow>
          \amp \ = \ \lim_{\D x \to 0}\frac{f(x_0+\D
          x,y_0)-f(x_0,y_0)}{\D x}
        </mrow>
        <mrow>
          \amp \ = \ \fderiv fx(x_0,y_0) \,
        </mrow>
      </md>.
    </p>
    <p>
      In the second case, <m>\D z = i \, \D y</m> and
      <md>
        <mrow>
          f'(z_0) \amp \ = \ \lim_{i \, \D y \to 0}\frac{f(z_0+i\D y) -
          f(z_0)}{i \, \D y}
        </mrow>
        <mrow>
          \amp \ = \ \lim_{\D y \to
          0}\frac1i\frac{f(x_0,y_0+\D y)-f(x_0,y_0)}{\D y}
        </mrow>
        <mrow>
          \amp \ = \ -i \,
          \fderiv fy(x_0,y_0) \,
        </mrow>
      </md>.
    </p>
    <p>
      Thus we have shown that <m>f'(z_0) = f_x(z_0) = -if_y(z_0)</m>.
    </p>
    <p>
      (b) Suppose the Cauchy<ndash/>Riemann equation <xref
      ref="complexcr"/> holds and the partial derivatives <m>f_x</m>
      and <m>f_y</m> are continuous in an open disk centered at
      <m>z_0</m>. 
      Our goal is to prove that <m>f'(z_0) = f_x(z_0)</m>.
      By <xref ref="complexcr"/>,
      <md>
        <mrow>
          f_x(z_0) \amp \ = \ \frac{\D x + i \, \D y}{\D z}\, f_x(z_0)
        </mrow>
        <mrow>
          \amp \ = \ \frac{\D x}{\D z}\, f_x(z_0) + \frac{\D y}{\D z}\, i \,
          f_x(z_0)
        </mrow>
        <mrow>
          \amp \ = \ \frac{\D x}{\D z}\, f_x(z_0) + \frac{\D y}{\D z}\,
          f_y(z_0) \,
        </mrow>
      </md>.
    </p>
    <p>
      On the other hand,
      we can rewrite the difference quotient for <m>f'(z_0)</m> as
      <md>
        <mrow>
          \amp\frac{f(z_0+\D z)-f(z_0)}{\D z}\amp
        </mrow>
        <mrow>
          \amp \ = \ \frac{f(z_0+\D
          z)-f(z_0+\D x) + f(z_0+\D x) - f(z_0)}{\D z}
        </mrow>
        <mrow>
          \amp \ = \ \frac{f(z_0+\D x+i\D y)-f(z_0+\D x)}{\D z} 
          + \frac{f(z_0+\D x) - f(z_0)}{\D z} \,
        </mrow>
      </md>.
    </p>
    <p>
      Thus
      <md>
        <mrow>
          \amp\lim_{\D z\to0}\frac{f(z_0+\D z)-f(z_0)}{\D z} - f_x(z_0)
        </mrow>
        <mrow>
          \amp = \lim_{\D z\to0} \frac{\D y}{\D
          z}\left(\frac{f(z_0+\D x+i\D y)-f(z_0+\D x)}{\D y} -
          f_y(z_0)\right)
        </mrow>
        <mrow xml:id="cauchyriemlimit" number="yes">
        \amp \qquad + \lim_{\D z\to0} \frac{\D x}{\D
        z}\left(\frac{f(z_0+\D x) - f(z_0)}{\D x} - f_x(z_0)\right)
        </mrow>
      </md>.
    </p>
    <p>
      We claim that both limits on the right-hand side are <m>0</m>,
      so we have achieved our set goal.
      The fractions <m>\frac{ \D x}{ \D z }</m> and
      <m>\frac{ \D y }{ \D z }</m> are bounded in absolute value by <m>1</m>,
      so we just need to see that the limits of the expressions in
      parentheses are <m>0</m>. 
      The second term on the right-hand side of <xref
      ref="cauchyriemlimit"/> has a limit of <m>0</m> since, 
      by definition,
      <me>
        f_x(z_0) \ = \ \lim_{\D x\to0}\frac{f(z_0+\D x) - f(z_0)}{\D x}
      </me>
      and taking the limit here as
      <m>\D z\to0</m> is the same as taking the limit as <m>\D x\to0</m>.
    </p>
    <p>
      We cannot do something equivalent for the first term in <xref
      ref="cauchyriemlimit"/>, 
      since now both <m>\D x</m> and <m>\D y</m> are involved,
      and both change as <m>\D z\to0</m>.
      Instead we apply the Mean-Value <xref ref="realmeanvalue"/> for
      real functions,<fn>  
      We collect several theorems from calculus,
      such as the Mean-Value Theorem for real-valued functions,
      in the Appendix.
      </fn> to the real and imaginary parts <m>u(z)</m> and
      <m>v(z)</m> of <m>f(z)</m>. 
      <xref ref="realmeanvalue"/>
      gives real numbers <m>0\lt a,b\lt 1</m> such that
      <md>
        <mrow>
        \frac{u(x_0+\D x, \, y_0+\D y)-u(x_0+\D x, \, y_0)}{\D y} \amp
        \ = \ u_y(x_0+\D x, \, y_0+a \, \D y)
        </mrow>
        <mrow>
        \frac{v(x_0+\D x, \, y_0+\D y)-v(x_0+\D x, \, y_0)}{\D y} \amp
        \ = \ v_y(x_0+\D x, \, y_0+b \, \D y) \,
        </mrow>
      </md>.
    </p>
    <p>
      Thus
      <md>
        <mrow>
          \amp \frac{f(z_0+\D x+ i \D y)-f(z_0+\D x)}{\D y} -
          f_y(z_0)
        </mrow>
        <mrow>
          \amp = \left( \frac{ u(x_0 + \D x, y_0 + \D y) - u(x_0
          + \D x, y_0) }{ \D y } - u_y(z_0) \right) 
        </mrow>
        <mrow>
          \amp \quad + i \left(
          \frac{ v(x_0 + \D x, y_0 + \D y) - v(x_0 + \D x, y_0) }{
          \D y } - v_y(z_0) \right)
        </mrow>
        <mrow xml:id="eq_laststepcauchyr" number="yes">
          \amp = \left(u_y(x_0+\D x, y_0+a \D y)-u_y(x_0,
          y_0)\right)
        </mrow>
        <mrow>
          \amp \quad + i\left(v_y(x_0+\D x, y_0+b \D y)-v_y(x_0,
          y_0)\right) 
        </mrow>
      </md>.
    </p>
    <p>
      Because <m>u_y</m> and <m>v_y</m> are continuous at <m>(x_0,y_0)</m>,
      <md>
        <mrow>
          \lim_{ \D z \to 0 } u_y(x_0+\D x, \, y_0+a \, \D y) \amp \ = \
          u_y(x_0, \, y_0)
        </mrow>
        <mrow>
          \lim_{ \D z \to 0 } v_y(x_0+\D x, \, y_0+b \, \D y) \amp \ = \
          v_y(x_0, \, y_0) \, 
        </mrow>
      </md>,
      and so <xref ref="eq_laststepcauchyr"/> goes to 0 as <m>\D z \to 0</m>,
      which we set out to prove.
    </p>
  </proof>
</section>
