<?xml version="1.0" encoding="utf-8"?>

<section xml:id="sec_limitsandcontinuity">
  <title>Limits and Continuity</title>
  <definition>
    <statement>
      <p>
        A <em>(complex) function</em>
        <m>f</m> is a map from a subset <m>G \subseteq \C</m> to
        <m>\C</m>; 
        in this situation we will write
        <m>f : G \to \C</m> and call <m>G</m> the <em>domain</em>
        of <m>f</m>.
        <idx><h>domain</h></idx>
        <idx><h>function</h></idx>
        This means that each element <m>z \in G</m> gets mapped to
        exactly one complex number, 
        called the <em>image</em> of <m>z</m> and usually denoted by
        <m>f(z)</m>. 
        <idx><h>image</h><h>of a point</h></idx>
      </p>
    </statement>
  </definition>
  <p>
    So far there is nothing that makes complex functions any more
    special than, say, 
    functions from <m>\R^m</m> to <m>\R^n</m>.
    In fact, we can construct many familiar looking functions from the
    standard calculus repertoire, 
    such as <m>f(z)=z</m> (the <em>identity map</em>), <idx><h>identity map</h></idx>
    <m>f(z)=2z+i</m>, <m>f(z)=z^3</m>,
    or <m>f(z) = \frac 1 z</m>.
    The former three could be defined on all of <m>\C</m>,
    whereas for the latter we have to exclude the origin <m>z=0</m>
    from the domain. 
    On the other hand,
    we could construct some functions that make use of a certain
    representation of <m>z</m>, 
    for example, <m>f(x,y) = x-2iy</m>,
    <m>f(x,y) = y^2-ix</m>, or <m>f(r,\phi) = 2r \, e^{ i (\phi + \pi)
    }</m>. 
  </p>
  <p>
    Next we define limits of a function.
    The philosophy of the following definition is not restricted to
    complex functions, 
    but for sake of simplicity we state it only for those functions.
        <idx><h>limit</h><h>of a function</h></idx>
  </p>
  <definition>
    <statement>
      <p>
        Suppose <m>f: G \to \C</m> and <m>z_0</m> is an accumulation point
        of <m>G</m>.
        <idx><h>accumulation point</h></idx>
        If <m>w_0</m> is a complex number such that for every
        <m>\epsilon>0</m> we can find <m>\gd>0</m> so that,
        for all <m>z\in G</m> satisfying
        <m>0 \lt  \left| z - z_0 \right| \lt  \gd</m>,
        we have <m>\left| f(z) - w_0 \right| \lt  \epsilon</m>,
        then <m>w_0</m> is the <em>limit</em>
        of <m>f</m> as <m>z</m> approaches <m>z_0</m>; in short,
        <me>
          \lim_{ z \to z_0 } f(z) \ = \ w_0 \, 
        </me>.
      </p>
    </statement>
  </definition>

  <p>
    This definition is the same as is found in most calculus texts.
    The reason we require that <m>z_0</m> is an accumulation point of
    the domain is just that we need to be sure that there are points
    <m>z</m> of the domain that are arbitrarily close to <m>z_0</m>.
    Just as in the real case, our definition (i.e., the part that says
    <m>0\lt \abs{z-z_0}</m>) does not require that <m>z_0</m> is in
    the domain of <m>f</m> and, if <m>z_0</m> is in the domain of
    <m>f</m>, the definition explicitly ignores the value of
    <m>f(z_0)</m>.
  </p>
  
  <example xml:id="exam_limitexists">
    <statement>
      <p>
        Let's prove that <m>\ds \lim_{ z \to i } z^2 = -1</m>.
      </p>
      <p>
        Given <m>\epsilon > 0</m>, we need to determine <m>\gd > 0</m>
        such that <m>0 \lt |z-i| \lt \gd</m> implies <m>|z^2 + 1| \lt
        \epsilon</m>.  We rewrite
        <me>
          \left| z^2 + 1 \right| \ = \ \left| z-i \right| \left| z+i
          \right| \ \lt  \ \gd \left| z+i \right| \,
        </me>.
      </p>
      <p>
        If we choose <m>\gd</m>, say,
        smaller than 1 then the factor <m>|z+i|</m> on the right can
        be bounded by 3 
        (draw a picture!).
        This means that any <m>\gd \lt  \min \{ \frac \epsilon 3, 1
        \}</m> should do the trick: 
        in this case, <m>0 \lt  |z-i| \lt  \gd</m> implies
        <me>
          \left| z^2 + 1 \right| \ \lt  \ 3 \gd \ \lt  \ \epsilon \,
        </me>.
      </p>
      <p>
        This was a proof written out in a way one might come up with it.
        Here's a short, neat version:
      </p>
      <p>
        Given <m>\epsilon > 0</m>,
        choose <m>0 \lt  \gd \lt  \min \{ \frac \epsilon 3, 1 \}</m>.
        Then <m>0 \lt  |z-i| \lt  \gd</m> implies
        <me>
          \left|z+i\right| \ = \ \left|z-i + 2i\right| \ \le \ \left|
          z-i \right| + \left| 2i \right| \ \lt  \ 3 \,
        </me>
        from which we conclude that
        <me>
          \left| z^2 - (-1) \right| \ = \ \left| z^2 + 1 \right| \ = \
          \left| z-i \right| \left| z+i \right| \ \lt  \ 3 \gd \ \lt
          \ \epsilon \, 
        </me>.
        This proves <m>\lim_{ z \to i } z^2 = -1</m>. 
      </p>
    </statement>
  </example>
    <sage>
      <input>
        f(z) = sin(z)/z
        f.limit(z=0)
      </input>
      <output>
        z |--> 1
      </output>
    </sage>
  <p>
    Just as in the real case, the limit <m>w_0</m> is unique if it
    exists (see <xref ref="ex_limitunique"/>).  It is often
    useful to investigate limits by restricting the way the point
    <m>z</m> approaches <m>z_0</m>.  The following result is a direct
    consequence of the definition.
  </p>
  
  <proposition xml:id="restrictedlimit">
    <statement>
      <p>
        Suppose <m>f: G \to \C</m> and <m>\lim_{z\to z_0}f(z) =
        w_0</m>.  Suppose <m>\widetilde G \subseteq G</m> and
        <m>z_0</m> is an accumulation point of <m>\widetilde G</m>.
        If <m>\widetilde f</m> is the restriction of <m>f</m> to
        <m>\widetilde G</m>, then <m>\lim_{z\to z_0} \widetilde
        f(z)</m> exists and has the value <m>w_0</m>.
      </p>
    </statement>
  </proposition>

  <p>
    The definition of <em>limit</em> in the complex domain has to be
    treated with a little more care than its real companion; this is
    illustrated by the following example.
  </p>

  <example xml:id="exam_limitdoesnotexist">
    <statement>
      <p>
        The limit of <m>\frac{\, \overline z \, } z</m> as <m>z \to
        0</m> does not exist.
      </p>
      <p>
        To see this, we try to compute this limit as <m>z \to 0</m> on
        the real and on the imaginary axis.  In the first case, we can
        write <m>z = x \in \R</m>, and hence
        <me>
          \lim_{ z \to 0 } \frac{ \, \overline z \, }{ z } \ = \ \lim_{ x
          \to 0 } \frac{ \, \overline x \, }{ x } \ = \ \lim_{ x \to 0 }
          \frac{ x }{ x } \ = \ 1 \, 
        </me>.
      </p>
      <p>
        In the second case,
        we write <m>z = iy</m> where <m>y \in \R</m>, and then
        <me>
          \lim_{ z \to 0 } \frac{ \, \overline z \, }{ z } \ = \ \lim_{ y
          \to 0 } \frac{ \, \overline{iy} \, }{ iy } \ = \ \lim_{ y \to 0
          } \frac{ -iy }{ iy } \ = \ -1 \, 
        </me>.
      </p>
      <p>
        So we get a different
        <q>limit</q>
        depending on the direction from which we approach 0.
        <xref ref="restrictedlimit">Proposition</xref>
        then implies that the limit of
        <m>\frac{\, \overline z \, } z</m> as <m>z \to 0</m> does not
        exist.
      </p>
    </statement>
  </example>

  <p>
    On the other hand,
    the following usual limit rules are valid for complex functions;
    the proofs of these rules are everything but trivial and make for
    nice practice (see <xref ref="ex_limits"/>);
    as usual, we give a sample proof.
  </p>
  
  <proposition xml:id="limits">
    <statement>
      <p>
        Let <m>f</m> and <m>g</m> be complex functions with domain
        <m>G</m>, let <m>z_0</m> be an accumulation point of <m>G</m>,
        and let <m>c \in \C</m>.  If <m>\lim_{ z \to z_0 } f(z)</m>
        and <m>\lim_{ z \to z_0 } g(z)</m> exist, then
        <ol marker="(a) ">
          <li xml:id="limitsadd">
            <p>
              <m>\displaystyle
              \lim_{ z \to z_0 } \left( f(z) + c g(z) \right)
              = \lim_{ z \to z_0 } f(z) + c \lim_{ z \to z_0 } g(z) \,
              </m>.
            </p>
          </li>
          <li xml:id="limitsmultiply">
            <p>
              <m>\displaystyle
              \lim_{ z \to z_0 } \left( f(z) \cdot g(z) \right) \ = \
              \lim_{ z \to z_0 } f(z) \cdot \lim_{ z \to z_0 } g(z) \,
              </m>.
            </p>
          </li>
          <li>
            <p>
              <m>\displaystyle
              \lim_{ z \to z_0 } \frac{ f(z) }{ g(z) } \ = \ \frac{
              \lim_{ z \to z_0 } f(z) }{ \lim_{ z \to z_0 } g(z) } \,
              </m>.
            </p>
          </li>
        </ol>
      </p>
      <p>
        where in the last identity we also require that <m>\lim_{ z
        \to z_0 } g(z) \neq 0</m>. 
      </p>
    </statement>
    <proof>
      <p>We will prove (<xref text="local" ref="limitsadd"/>).
      Assume that <m>c \ne 0</m>
      (otherwise there is nothing to prove),
      and let <m>L = \lim_{ z \to z_0 } f(z)</m> and <m>M = \lim_{ z
      \to z_0 } g(z)</m>. 
      Then we know that, given <m>\epsilon > 0</m>,
      we can find <m>\delta_1, \delta_2 > 0</m> such that
      <me>
        0 \lt  |z-z_0| \lt  \delta_1 \text{ implies } \left| f(z) - L
        \right| \lt  \frac \epsilon 2 
      </me>
      and
      <me>
        0 \lt  |z-z_0| \lt  \delta_2 \text{ implies } \left| g(z) - M
        \right| \lt  \frac \epsilon {2|c|} \, 
        </me>.
      </p>
      <p>
        Thus, choosing <m>\delta = \min \{ \delta_1, \delta_2 \}</m>,
        we infer that <m>0 \lt  |z-z_0| \lt  \delta</m> implies
        <me>
          \left| (f(z) + c \, g(z)) - (L+c \, M) \right| \ \le \ \left|
          f(z) - L \right| + |c| \left| g(z) - M \right| \ \lt  \
          \epsilon \, 
          </me>.
      </p>
      <p>
        Here we used the triangle inequality
        (<xref ref="lem_triangleineq">Proposition</xref>).
        This proves that <m>\lim_{ z \to z_0 } (f(z) + c \, g(z)) = L+c
        \, M</m>, 
        which was our claim.
      </p>
    </proof>
  </proposition>
  
  <p>
    Because the definition of the limit is somewhat elaborate,
    the following fundamental definition looks almost trivial.
    <idx><h>trivial</h></idx>
  </p>
  
  <definition>
    <statement>
      <p>
        Suppose <m>f: G \to \C</m>.
        If <m>z_0 \in G</m> and either <m>z_0</m> is an isolated point
        of <m>G</m> or 
        <me>
          \lim_{ z \to z_0 } f(z) \ = \ f(z_0)
        </me>
        then <m>f</m> is <em>continuous</em>
        at <m>z_0</m>.
        <idx><h>continuous</h></idx>
        More generally, <m>f</m> is <em>continuous</em>
        on <m>E \subseteq G</m> if <m>f</m> is continuous at every
        <m>z \in E</m>. 
      </p>
    </statement>
  </definition>

  <p>
    However, in almost all proofs using continuity it is necessary to
    interpret this in terms of <m>\epsilon</m>'s and <m>\delta</m>'s.
    So here is an alternate definition:
  </p>
  
  <definition>
    <statement>
      <p>
        Suppose <m>f: G \to \C</m> and <m>z_0 \in G</m>.
        Then <m>f</m> is <em>continuous</em>
        at <m>z_0</m> if, for every positive real number
        <m>\epsilon</m>, there is a positive real number <m>\delta</m>
        so that 
        <me>
          |\,f(z)-f(z_0)\,| \lt  \epsilon \;\text{ for all } \; z\in G
          \; \text{ satisfying } \; |\,z-z_0\,| \lt  \delta\, 
        </me>.
        <idx><h>continuous</h></idx>
      </p>
    </statement>
  </definition>

  <p>
    See <xref ref="ex_continuitydefs"/> for a proof that these
    definitions are equivalent. 
  </p>
  
  <example>
    <statement>
      <p>
        We already proved
        (in <xref ref="exam_limitexists"/>)
        that the function <m>f: \C \to \C</m> given by
        <m>f(z) = z^2</m> is continuous at <m>z = i</m>.
        You're invited
        (see <xref ref="ex_zsquaredcontinuous"/>)
        to extend our proof to show that,
        in fact, this function is continuous on <m>\C</m>. 
      </p>
      <p>
        On the other hand, let <m>g: \C \to \C</m> be given by 
        <me>
          g(z) := \begin{cases}\frac{\, \overline z \, } z \amp
          \text{ if }  z \ne 0 \, , \\ 1 \amp  \text{ if }  z = 0 \,
          . \end{cases} 
        </me>
        In <xref ref="exam_limitdoesnotexist"/>
        we proved that <m>g</m> is not continuous at <m>z = 0</m>.
        However, this is its only point of discontinuity
        (see <xref ref="ex_zbaroverzcont"/>). 
      </p>
    </statement>
  </example>

  <p>
    Just as in the real case, we can
    <q>take the limit inside</q>
    a continuous function, by considering composition of functions.
  </p>
  
  <definition>
    <statement>
      <p>
        The <em>image</em> of the function
        <m>g: G \to \C</m> is the set
        <m>\left\{ g(z) : \, z \in G \right\}
        </m>. 
        <idx><h>image</h><h>of a function</h></idx>
        If the image of <m>g</m> is contained in the domain of another
        function <m>f : H \to \C</m>, 
        we define the <em>composition</em>
        <m>f \circ g : G \to \C</m> through
        <me>
          (f \circ g) (z) \ := \ f(g(z)) \,
        </me>.
        <idx><h>composition</h></idx>
      </p>
    </statement>
  </definition>
  
  <proposition xml:id="funoflimit">
    <statement>
      <p>
        Let <m>g : G \to \C</m> with image contained in <m>H</m>,
        and let <m>f : H \to \C</m>.
        Suppose <m>z_0</m> is an accumulation point of <m>G</m>,
        <m>\lim_{z\to z_0}g(z)=w_0\in H</m>,
        and <m>f</m> is continuous at <m>w_0</m>.
        Then <m>\lim_{z\to z_0}f(g(z))=f(w_0)</m>; in short,
        <me>
          \lim_{z\to z_0} f(g(z)) \ = \ f\left(\lim_{z\to z_0}g(z)\right)
        </me>.
      </p>
    </statement>
    <proof>
      <p>
        Given <m>\epsilon > 0</m>, we know there is an <m>\eta > 0</m> such that
        <me>
          |w-w_0| \lt  \eta \text{ implies } \left| f(w) - f(w_0)
          \right| \lt  \epsilon \, 
          </me>.
        For this <m>\eta</m>,
        we also know there is a <m>\delta > 0</m> such that
        <me>
          0 \lt  |z-z_0| \lt  \delta \text{ implies } \left| g(z) -
          w_0 \right| \lt  \eta \, 
          </me>.
        Stringing these two implications together gives that
        <me>
          0 \lt  |z-z_0| \lt  \delta \text{ implies } \left| f(g(z)) -
          f(w_0) \right| \lt  \epsilon \, 
          </me>.
        We have thus proved that <m>\lim_{z\to z_0}f(g(z))=f(w_0)</m>.
      </p>
    </proof>
  </proposition>
</section>
