<?xml version="1.0" encoding="utf-8"?>

<section xml:id="sec_logexp"
         xmlns:xi="http://www.w3.org/2001/XInclude">
  <title>Logarithms and Complex Exponentials</title>
  <p>
    The complex logarithm
    is the first function we'll encounter that is of a somewhat tricky
    nature.
    <idx><h>logarithm</h></idx>
    It is motivated as an inverse to the exponential function, that
    is, 
    we're looking for a function <m>\fLog</m> such that
    <men xml:id="eq_expinv">
      \exp ( \fLog(z) ) \ = \ z \ = \ \fLog ( \exp z ) \,
    </men>.
    <idx><h>function</h><h>logarithmic</h></idx> 
  </p>
  <p>
    But because <m>\exp</m> is not one-to-one,
    this is too much to hope for.
    In fact, given a function <m>\fLog</m> that satisfies the first
    equation in <xref ref="eq_expinv"/>,
    the function <m>f(z) = \fLog(z) + 2 \pi i</m> does as well,
    and so there cannot be an inverse of <m>\exp</m>
    (which would have to be unique).
    On the other hand,
    <m>\exp</m> becomes one-to-one if we restrict its domain,
    so there is hope for a logarithm if we are careful about its
    construction and about its domain.
  </p>
  <definition>
    <statement>
      <p>
        Given a region <m>G</m>,
        any continuous function <m>\fLog : G \to \C</m> that satisfies
        <m>\exp(\fLog z) = z</m> is 
        <em>a branch of the logarithm
        (on <m>G</m>)</em>.
        <idx><h>branch of the logarithm</h></idx>
      </p>
    </statement>
  </definition>
  <p>
    To make sure this definition is not vacuous, let's write,
    as usual, <m>z = r \, e^{i \phi}</m>,
    and suppose that <m>\fLog z = u(z) + i \, v(z)</m>.
    Then for the first equation in <xref ref="eq_expinv"/> to hold, we
    need 
    <me>
      \exp ( \fLog z ) \ = \ e^{u} e^{i v} \ = \ r \, e^{i \phi} \ = \ z \,
    </me>,
    that is, <m>e^{u} = r</m> and <m>e^{i v} = e^{i \phi}</m>.
    The latter equation is equivalent to
    <m>v = \phi + 2 \pi k</m> for some <m>k \in \Z</m>,
    and denoting the natural logarithm of the positive real number
    <m>x</m> by <m>\ln(x)</m>, 
    the former equation is equivalent to <m>u = \ln |z|</m>.
    A reasonable definition of a logarithm function <m>\fLog</m> would
    hence be 
    <m>\fLog z = \ln |z| + i \fArg z</m> where <m>\fArg z</m> gives
    the argument for the complex number <m>z</m> according to some
    convention<mdash/>here is an example.
  </p>
  <definition>
    <statement>
      <p>
        Let <m>\Arg z</m>
        denote the unique argument of <m>z \ne 0</m> that lies in
        <m>(-\pi, \pi]</m> 
        (the <em>principal argument
        of <m>z</m></em>).
        <idx><h>Arg</h></idx>
        <idx><h>principal argument</h></idx>
        Then the <em>principal logarithm
        </em> is the function <m>\Log: \C \setminus \{ 0 \} \to \C</m>
        defined through 
        <me>
          \Log(z) := \ln |z| + i \Arg(z) \,
        </me>.
        <idx><h>principal logarithm</h></idx>
        <idx><h>Log</h></idx>
      </p>
    </statement>
  </definition>
  <example>
    <statement>
      <p>
        Here are a few evaluations of <m>\Log</m> to illustrate this function:
        <md>
          <mrow>\Log(2) \amp \ = \ \ln(2) + i \Arg(2) \ = \ \ln(2)</mrow>
          <mrow>\Log(i) \amp \ = \ \ln(1) + i \Arg(i) \ = \ \frac{ \pi i }{
          2 }</mrow> 
          <mrow>\Log(-3) \amp \ = \ \ln(3) + i \Arg(-3) \ = \ \ln(3) + \pi
          i</mrow> 
          <mrow>\Log(1-i) \amp \ = \ \ln( \sqrt 2 ) + i \Arg(1-i) \ = \
          \frac 1 2 \ln(2) - \frac{ \pi i }{ 4 } \, </mrow> 
        </md>.
      </p>
    </statement>
  </example>
  <p>
    <c>SageMath</c> computes <q>our</q> principal logarithm.
  </p>
    <sage>
      <input>
        real(log(1-i))
      </input>
      <output>
        log(sqrt(2))
      </output>
    </sage>
    <sage>
      <input>
        imaginary(log(1-i))
      </input>
      <output>
        -1/4*pi
      </output>
    </sage>
  <p>
    The principal logarithm is not continuous on the negative part of
    the real line, 
    and so <m>\Log</m> is a branch of the logarithm on <m>\C \setminus
    \R_{ \le 0 }</m>. 
    Any branch of the logarithm on a region <m>G</m> can be similarly
    extended to a function defined on <m>\overline G \setminus \{ 0
    \}</m>. 
    Furthermore,
    the evaluation of any branch of the logarithm at a specific
    <m>z_0</m> can differ from 
    <m>\Log(z_0)</m> only by a multiple of <m>2 \pi i</m>;
    the reason for this is once more the periodicity of the
    exponential function. 
  </p>
  <p>
    So what about the second equation in <xref ref="eq_expinv"/>,
    namely, 
    <m>\fLog (\exp z) = z</m>?
    Let's try the principal logarithm:
    if <m>z=x+iy</m> then
    <md>
      <mrow>
        \Log ( \exp z ) \amp \ = \ \ln | e^x e^{iy} | + i \Arg ( e^x
        e^{iy} )
      </mrow>
      <mrow>
        \amp \ = \ \ln e^x + i \Arg ( e^{iy} )
      </mrow>
      <mrow>
        \amp \ = \ x + i \Arg ( e^{iy} )
      </mrow>
    </md>.
  </p>
  <p>
    The right-hand side is equal to <m>z=x+iy</m> if and only if <m>y
    \in (-\pi, \pi]</m>. 
    Something similar will happen with any other branch <m>\fLog</m>
    of the logarithm<mdash/>there will always be many <m>z</m>'s for
    which <m>\fLog ( \exp z ) \ne z</m>. 
  </p>
  <p>
    A warning sign pointing in a similar direction concerns the
    much-cherished real logarithm rule <m>\ln(xy) = \ln(x) +
    \ln(y)</m>; 
    it has no analogue in <m>\C</m>.
    For example,
    <me>
      \Log(i) + \Log(i-1) \ = \ i \, \tfrac \pi 2 + \ln \sqrt 2 + \tfrac
      {3 \pi i} 4 \ = \ \tfrac 1 2 \ln 2 + \tfrac {5 \pi i} 4 
    </me>
    but
    <me>
      \Log(i(i-1)) \ = \ \Log(-1-i) \ = \ \tfrac 1 2 \ln 2 - \tfrac {3 \pi
      i} 4 \, 
    </me>.
  </p>
  <p>
    The problem is that we need to come up with an argument convention
    to define a logarithm and then stick to this convention. 
    There is quite a bit of subtlety here;
    e.g., the multi-valued map
    <me>
      \arg z \ := \ \text{ all possible arguments of }  z
    </me>
    gives rise to a multi-valued logarithm via
    <me>
      \log z \ := \ \ln |z| + i \arg z \,
    </me>.
    <idx><h>arg</h></idx>
    <idx><h>log</h></idx>
  </p>
  <p>
    Neither <m>\arg</m> nor <m>\log</m> is a function,
    yet <m>\exp ( \log z ) = z</m>.
    We invite you to check this thoroughly;
    in particular,
    you should note how the periodicity of the exponential function
    takes care of the multi-valuedness of <m>\log</m>. 
  </p>
  <p>
    To end our discussion of complex logarithms on a happy note,
    we prove that <em>any</em> branch of the logarithm has the
    <em>same</em> derivative;
    one just has to be cautious with regions of holomorphicity.
  </p>
  <proposition>
    <statement>
      <p>
        If <m>\fLog</m> is a branch of the logarithm on <m>G</m>, then
        <m>\fLog</m> is differentiable on <m>G</m> with 
        <me>
          \frac{ d }{ \diff{z} } \fLog(z) \ = \ \frac 1 z \,
        </me>.
      </p>
    </statement>
  </proposition>
  <proof>
    <p>
      The idea is to apply <xref ref="inversederivative"/>
      to <m>\exp</m> and <m>\fLog</m>,
      but we need to be careful about the domains of these functions.
      Let <m>H := \{ \fLog(z) : \, z \in G \}</m>,
      the image of <m>\fLog</m>.
      We apply <xref ref="inversederivative">Proposition</xref>
      with <m>f: H \to G</m> given by <m>f(z) = \exp(z)</m> and
      <m>g: G \to H</m> given by <m>g(z) = \fLog(z)</m>;
      note that <m>g</m> is continuous,
      and <xref ref="ex_logexpinv"/>
      checks that <m>f</m> and <m>g</m> are inverses of each other.
      Thus <xref ref="inversederivative"/> gives
      <me>
        \fLog'(z) \ = \ \frac 1 { \exp' ( \fLog z ) } \ = \ \frac 1 { \exp (
        \fLog z ) } \ = \ \frac 1 z \,
      </me>.
    </p>
  </proof>
  <p>
    We finish this section by defining complex exponentials.
  </p>
  <definition>
    <statement>
      <p>
        Given <m>a, b \in \C</m> with <m>a \ne 0</m>,
        the <em>principal value of <m>a^b</m><idx><h>principal value
        of <m>a^b</m></h></idx> 
        </em> is defined as
        <me>
          a^b \ := \ \exp ( b \Log(a)) \,
        </me>.
      </p>
    </statement>
  </definition>
  <p>
    Naturally, we can just as well define <m>a^b</m> through a
    different branch of the logarithm; 
    our convention is that we use the principal value unless otherwise
    stated. 
    <xref ref="singlevaluedexp"/>
    explores what happens when we use the multi-valued <m>\log</m> in
    the definition of <m>a^b</m>. 
  </p>
  <p>
    One last remark:
    it now makes sense to talk about the function <m>f(z) = e^z</m>,
    where <m>e</m>
    is <em>Euler's
    <fn>
      Named after Leonard Euler (1707<ndash/>1783).
      Continuing our footnote on p.
      <xref ref="fn_eulerformula"/>
      we have now honestly established
      <em>Euler's formula</em>
      <m>e^{ 2 \pi i } = 1</m>.
    </fn>
    number</em> and can be defined, for example,
    as <m>e = \lim_{n \to \infty} \left( 1 + \frac 1 n \right)^n</m>.
    <idx><h>e@<m>e</m></h></idx>
    In calculus we can prove the equivalence of the real exponential function
    (as given, for example, through a power series)
    and the function <m>f(x) = e^x</m>.
    With our definition of <m>a^z</m>,
    we can now make a similar remark about the complex exponential function.
    Because <m>e</m> is a positive real number and hence <m>\Arg e = 0</m>,
    <md>
      <mrow>
        e^z \amp \ = \ \exp ( z \Log(e))
      </mrow>
      <mrow>
        \amp \ = \ \exp \left( z \left( \ln |e| + i
        \Arg(e) \right) \right)
      </mrow>
      <mrow>
        \amp \ = \ \exp \left( z \ln(e) \right)
      </mrow>
      <mrow>
        \amp \ = \ \exp
        \left( z \right)
      </mrow>
    </md>.
  </p>
  <p>
    A word of caution:
    this only works out this nicely because we have carefully defined
    <m>a^b</m> for complex numbers. 
    Using a different branch of logarithm in the definition of
    <m>a^b</m> can easily lead to <m>e^z \ne \exp(z)</m>. 
  </p>
    <sage>
      <input>
        real(i^i)
      </input>
      <output>
        e^(-1/2*pi)
      </output>
    </sage>
    <sage>
      <input>
        imaginary(i^i)
      </input>
      <output>
        0
      </output>
    </sage>
</section>
