<?xml version="1.0" encoding="utf-8"?>

<section xml:id="sec_powerseriesholom">
  <title>Power Series and Holomorphic Functions</title>
  <p>
    Here is the first
    (and easier)
    half of the first goal we just announced.
  </p>
  <theorem xml:id="thm_powerholomorphic">
    <statement>
      <p>
        Suppose <m>f(z) = \s c_k \left( z - z_0 \right)^k</m> has
        radius of convergence <m>R>0</m>. 
        Then <m>f</m> is holomorphic in <m>D[z_0, R]</m>.
      </p>
    </statement>
    <proof>
      <p>
        <xref ref="powseriescontinuous"/>
        says that <m>f</m> is continuous in <m>D[z_0, R]</m>.
        Given any closed piecewise smooth path <m>\gamma \subset
        D[z_0, R]</m>, 
        <xref ref="powseriesintegral"/> gives <m>\int_\gg f = 0</m>.
        Now apply Morera's theorem
        (<xref ref="morera"/>).
      </p>
    </proof>
  </theorem>
  <p>
    A special case of this result concerns power series with infinite
    radius of convergence: 
    those represent entire functions.
  </p>
  <p>
    Now that we know that power series are differentiable in their
    regions of convergence, 
    we can ask how to find their derivatives.
    The next result says that we can simply differentiate the series
    term by term. 
  </p>
  <theorem xml:id="powerderivative">
    <statement>
      <p>
        Suppose <m>f(z) = \s c_k ( z - z_0 )^k</m> has radius of
        convergence <m>R>0</m>. 
        Then 
        <me>
          f'(z) \ = \ \sum_{ k \geq 1 } k \, c_k ( z - z_0 )^{k-1}
          \;\text{ for any } \;z\in D[z_0, R] \, 
        </me>,
        and the radius of convergence of this power series is
        also <m>R</m>.
        <idx><h>power series</h><h>differentiation of</h></idx>
      </p>
    </statement>
    <proof>
      <p>
        If <m>z\in D[z_0,R]</m> then <m>|z-z_0|\lt R</m>,
        so we can choose <m>R_1</m> so that <m>|z-z_0|\lt R_1\lt R</m>.
        Then the circle <m>\gg:=C[z_0,R_1]</m> lies in
        <m>D[z_0,R]</m> and <m>z</m> is inside <m>\gg</m>.
        Since <m>f</m> is holomorphic in
        <m>D[z_0,R]</m> we can use Cauchy's Integral Formula for <m>f'</m>
        (<xref ref="cauchyformula2"/>),
        as well as <xref ref="powseriesintegral"/>:
        <md>
          <mrow>f'(z) \amp \ = \ \frac{1}{2 \pi i} \int_\gg
          \frac{f(w)}{(w-z)^2} \, \diff{w} \ = \ \frac{1}{2 \pi i} \int_\gg
          \frac{1}{(w-z)^2} \s c_k (w-z_0)^k \, \diff{w}</mrow> 
          <mrow>\amp \ = \ \s c_k \, \frac{1}{2 \pi i} \int_\gg
          \frac{(w-z_0)^k}{(w-z)^2} \, \diff{w} \ = \ \s c_k
          \left.\frac{d}{\diff{w}} (w-z_0)^k\right|_{w=z}</mrow> 
          <mrow>\amp \ = \ \sum_{ k \ge 1 }  k \, c_k (z-z_0)^{k-1} </mrow>
        </md>.
      </p>
      <p>
        Note that we used <xref ref="cauchyformula2"/>
        <em>again</em> in the penultimate step,
        but now applied to the function <m>(z-z_0)^k</m>.
      </p>
      <p>
        The last statement of the theorem is easy to show:
        the radius of convergence of <m>f'(z)</m> is at least <m>R</m>
        (since we have shown that the series for <m>f'</m> converges
        whenever <m>\abs{z-z_0}\lt R</m>), 
        and it cannot be larger than <m>R</m> by comparison to the
        series for <m>f(z)</m>, 
        since the coefficients for
        <m>(z-z_0) \, f'(z)</m> are larger than the corresponding ones
        for<nbsp/><m>f(z)</m>. 
      </p>
    </proof>
  </theorem>
  <example xml:id="ex_exptaylor">
    <statement>
      <p>
        Let
        <me>
          f(z) \ = \ \s \frac{ z^k }{ k! } \,
        </me>.
      </p>
      <p>
        In <xref ref="exponentialfunctionradius"/>,
        we showed that <m>f</m> converges in <m>\C</m>.
        We claim that <m>f(z) = \exp(z)</m>,
        in analogy with the real exponential function.
        First, by <xref ref="powerderivative"/>,
        <me>
          f'(z) \ = \ \frac{d}{\diff{z}} \sum_{k \geq 0} \frac{z^k}{k!}
          \ = \ \sum_{k \geq 1} \frac{z^{k-1}}{(k-1)!} \ = \ \sum_{k \geq 0}
          \frac{z^k}{k!} \ = \ f(z)\, 
        </me>.
      </p>
      <p>
        Thus
        <md>
          <mrow> 
            \frac{ d }{ \diff{z} } \frac{ f(z) }{ \exp(z) }
            \ \amp= \ \frac{ d }{ \diff{z} } \left( f(z) \exp(-z) \right)
            \ = \ f'(z) \exp(-z) - f(z) \exp(-z)
          </mrow> 
          <mrow> 
            \amp = \ 0 \, 
          </mrow> 
        </md>,
        and so, by <xref ref="derivative0"/>,
        <m>\frac{ f(z) }{ \exp(z) }</m> is constant.
        Evaluating at <m>z=0</m> gives that this constant is 1, and so
        <m>f(z) = \exp(z)</m>. 
      </p>
    </statement>
  </example>
    <sage>
      <input>
        var('k', 'z')
        sum(z^k/factorial(k),k,0, +oo)
      </input>
      <output>
        e^z
      </output>
    </sage>
  <example xml:id="ex_sinpowerser">
    <statement>
      <p>
        We can use the power series expansion for <m>\exp(z)</m> to
        find power series for the trigonometric functions. 
        For instance,
        <md>
          <mrow>\sin z \amp \ = \ \frac{1}{2i}\left( \exp(iz) - \exp(-iz)
          \right) \ = \ \frac{1}{2i}\left( \sum_{k\geq
          0}\frac{(iz)^k}{k!} - \sum_{k\geq 0}\frac{(-iz)^k}{k!}
          \right)</mrow> 
          <mrow>\amp \ = \ \frac{1}{2i} \sum_{k\geq 0}\frac{1}{k!}\left(
          (iz)^k - (-1)^k(iz)^k \right) \ = \ \frac{1}{2i} \sum_{k\geq 0
          \text{ odd } }\frac{2(iz)^k}{k!}</mrow> 
          <mrow>\amp \ = \ \frac{1}{i} \sum_{j\geq
          0}\frac{(iz)^{2j+1}}{(2j+1)!} \ = \ \sum_{j\geq 0}\frac{i^{2j}
          \, z^{2j+1}}{(2j+1)!} \ = \ \sum_{j\geq
          0}\frac{(-1)^j}{(2j+1)!} \, z^{2j+1}</mrow> 
          <mrow>\amp \ = \ z - \frac{z^3}{3!} + \frac{z^5}{5!} -
          \frac{z^7}{7!} + \cdots \,</mrow> 
        </md>.
      </p>
      <p>
        Note that we are allowed to rearrange the terms of the two
        added sums because the corresponding series have infinite
        radii of convergence. 
      </p>
    </statement>
  </example>
    <sage>
      <input>
        var('z')
        taylor(sin(z),z,0,10)
      </input>
      <output>
        1/362880*z^9 - 1/5040*z^7 + 1/120*z^5 - 1/6*z^3 + z
      </output>
    </sage>
  <p>
    Naturally, <xref ref="powerderivative"/>
    can be repeatedly applied to <m>f'</m>,
    then to <m>f''</m>, and so on.
    The various derivatives of a power series can also be seen as
    ingredients of the series itself<mdash/>this is the statement of
    the following 
    <em>Taylor series expansion</em>.
    <idx><h>Taylor series expansion</h></idx>
    <fn>
      Named after Brook Taylor (1685<ndash/>1731).
    </fn>
  </p>
  <corollary xml:id="taylor">
    <statement>
      <p>
        Suppose <m>f(z) = \s c_k ( z - z_0 )^k</m> has a positive
        radius of convergence. 
        Then
        <me>
          c_k \ = \ \frac{ f^{(k)} (z_0) }{ k! } \,
        </me>.
      </p>
    </statement>
  </corollary>
  <proof>
    <p>
      For starters, <m>f(z_0)=c_0</m>.
      <xref ref="powerderivative">Theorem</xref> gives <m>f'(z_0)=c_1</m>.
      Applying the same theorem to <m>f'</m> gives
      <me>
        f''(z) \ = \ \sum_{ k \geq 2 } k (k-1) \, c_k \left( z - z_0
        \right)^{k-2} 
      </me>
      and so <m>f''(z_0) = 2 \, c_2</m>.
      A quick induction game establishes <m>f'''(z_0) = 6 \, c_3</m>,
      <m>f''''(z_0) = 24 \, c_4</m>, etc.
    </p>
  </proof>
  <p>
    Taylor's formula shows that the coefficients of any power series
    converging to <m>f</m> on some open disk <m>D</m> can be
    determined from the function <m>f</m> restricted to <m>D</m>. 
    It follows immediately that the coefficients of a power series are
    unique: 
  </p>
  <corollary xml:id="uniqueness">
    <statement>
      <p>
        If <m>\sum_{k\ge0}c_k \, (z-z_0)^k</m> and
        <m>\sum_{k\ge0}d_k \, (z-z_0)^k</m> are two power series that
        both converge to the same function on an open disk centered at
        <m>z_0</m>, 
        then <m>c_k=d_k</m> for all <m>k \ge 0</m>.
      </p>
    </statement>
  </corollary>
  <example xml:id="ex_expatpi">
    <statement>
      <p>
        We'd like to compute a power series expansion for
        <m>f(z) = \exp(z)</m> centered at <m>z_0 = \pi</m>.
        Since
        <me>
          f^{ (k) } (z_0) \ = \ \biggl. \exp(z) \biggr|_{ z=\pi } \ = \ e^\pi
        </me>,
      </p>
      <p>
        <xref ref="taylor"/>
        suggests that this power series is
        <me>
          \s \frac{ e^\pi }{ k! } \, (z-\pi)^k
        </me>,
        which converges for all <m>z \in \C</m>
        (essentially by
        <xref ref="exponentialfunctionradius"/>). 
      </p>
    </statement>
  </example>
  <p>
    We now turn to the second cornerstone result of this section,
    that a holomorphic function can be locally represented by a power series.
  </p>
  <theorem xml:id="thm_holomorphicpower">
    <statement>
      <p>
        Suppose <m>f</m> is a function holomorphic in <m>D[z_0, R]</m>.
        Then <m>f</m> can be represented as a power series centered at
        <m>z_0</m>, 
        with a radius of convergence <m>\ge R</m>:
        <me>
          f(z) \ = \ \s c_k ( z - z_0 )^k \qquad \text{ with }  \qquad
          c_k \ = \ \frac 1 {2 \pi i} \int_\gg \frac{ f(w) }{
          (w-z_0)^{k+1} } \, \diff{w} \, 
        </me>,
        where <m>\gg</m> is any positively oriented, simple, closed,
        piecewise smooth path in <m>D[z_0, R]</m> for which <m>z_0</m>
        is inside<nbsp/><m>\gg</m>.
      </p>
    </statement>
    <proof>
      <p>
        Let <m>g(z) := f(z+z_0)</m>;
        so <m>g</m> is a function holomorphic in <m>D[0,R]</m>.
        Given <m>z \in D[0,R]</m>, let <m>r := \frac{ |z|+R }{ 2 }</m>.
        By Cauchy's Integral Formula
        (<xref ref="cauchyformula"/>),
        <me>
          g (z) \ = \ \frac 1 {2 \pi i} \int_{C[0,r]} \frac{ g(w) }{ w-z }
          \, \diff{w} \, 
        </me>.
      </p>
      <p>
        The factor <m>\frac 1 {w-z}</m> in this integral can be expanded
        into a geometric series (note that 
        <m>w \in C[0,r]</m> and so <m>| \frac z w | \lt  1</m>):
        <me>
          \frac 1 {w-z} \ = \ \frac 1 w \, \frac 1 { 1 - \frac z w } \ = \
          \frac 1 w \s \left( \frac z w \right)^k 
        </me>
        which converges uniformly in the variable
        <m>w \in C[0,r]</m> by <xref ref="prob_geomseriesfunky"/>.
        Hence <xref ref="seriesintegral"/> applies:
        <md>
          <mrow>g (z) \amp \ = \ \frac{1}{2 \pi i} \int_{C[0,r]} \frac{
          g(w) }{ w-z } \, \diff{w}
          </mrow>
          <mrow> \amp \ = \ \frac{1}{2 \pi i} \int_{C[0,r]}
          g(w) \, \frac{1}{w} \s \left( \frac z w \right)^k \diff{w}
          </mrow>
          <mrow> \amp \ = \
          \s \left( \frac{1}{2 \pi i} \int_{C[0,r]} \frac{g(w)}{w^{k+1}}
          \, \diff{w} \right) z^k </mrow> 
        </md>.
      </p>
      <p>
        Now, since <m>f(z) = g(z-z_0)</m>,
        we apply a change of variables to obtain
        <me>
          f(z) \ = \ \s \left( \frac 1 {2 \pi i} \int_{C[z_0, r]} \frac{
          f(w) }{ (w-z_0)^{k+1} } \, \diff{w} \right) (z-z_0)^k 
          </me>.
      </p>
      <p>
        The only differences of this right-hand side to the statement of
        the theorem are the paths we're integrating over. 
        However, by Cauchy's <xref ref="cauchythm"/>,
        <me>
          \int_{C[z_0, r]} \frac{ f(w) }{ (w-z_0)^{k+1} } \, \diff{w} \ = \
          \int_\gg \frac{ f(w) }{ (w-z_0)^{k+1} } \, \diff{w} \,  
        </me>.
      </p>
    </proof>
  </theorem>
  <p>
    We note a remarkable feature of our proof:
    namely, if we are given a holomorphic function
    <m>f: G \to \C</m> and are interested in expanding <m>f</m> into a
    power series centered at <m>z_0 \in G</m>, 
    then we may maximize the radius of convergence <m>R</m> of this
    power series, 
    in the sense that its region of convergence reaches to the
    boundary of <m>G</m>. 
    Let's make this precise.
  </p>
  <definition>
    <statement>
      <p>
        For a region <m>G \subseteq \C</m> and a point <m>z_0 \in G</m>,
        we define the <em>distance of <m>z_0</m> to
        <m>\partial G</m></em>, the boundary of <m>G</m>,
        as the greatest lower bound of <m>\{ |z-z_0| : \, z \in
        \partial G \}</m>; 
        if this set is empty, we define the distance of <m>z_0</m> to
        <m>\partial G</m> to be<nbsp/><m>\infty</m>.
      </p>
    </statement>
  </definition>
  <p>
    What we have proved above, on the side, is the following.
  </p>
  <corollary xml:id="cor_powerseriesboundary">
    <statement>
      <p>
        If <m>f: G \to \C</m> is holomorphic and <m>z_0 \in G</m>,
        then <m>f</m> can be expanded into a power series centered at
        <m>z_0</m> whose radius of convergence is at least the
        distance of <m>z_0</m> to<nbsp/><m>\partial G</m>. 
      </p>
    </statement>
  </corollary>
  <example xml:id="ex_powerseriesboundary">
    <statement>
      <p>
        Consider <m>f: \C \setminus \{ \pm i \} \to \C</m> given by
        <m>f(z) := \frac 1 { z^2 + 1 }</m> and <m>z_0 = 0</m>. 
        <xref ref="cor_powerseriesboundary"/>
        says that the power series expansion of <m>f</m> at 0 will
        have radius of convergence 1. (Actually, 
        it says this radius is <em>at least</em>
        1, but it cannot be larger since <m>\pm i</m> are
        singularities of <m>f</m>.) In fact, 
        we can use a geometric series to compute this power series:
        <me>
          f(z) \ = \ \frac 1 { z^2 + 1 } \ = \ \s \left( -z^2 \right)^k \ = \
          \s (-1)^k \, z^{ 2k } 
        </me>,
        with radius of convergence 1.
      </p>
    </statement>
  </example>
  <p>
    <xref ref="cor_powerseriesboundary"/>
    is yet another example of a result that is plainly false when
    translated into <m>\R</m>; 
    see <xref ref="prob_powerseriesboundaryreal"/>.
  </p>
  <p>
    Comparing the coefficients of the power series obtained in
    <xref ref="thm_holomorphicpower"/>
    with those in <xref ref="taylor"/>,
    we arrive at the long-promised extension of
    <xref ref="cauchyformula"/>
    and <xref ref="cauchyformula2"/>.
  </p>
  <corollary xml:id="cauchyformula3">
    <statement>
      <p>
        Suppose <m>f</m> is holomorphic in the region <m>G</m> and
        <m>\gg</m> is a positively oriented, 
        simple, closed, piecewise smooth path,
        such that <m>w</m> is inside <m>\gg</m> and <m>\gg \sim_G 0</m>.
        Then <idx><h>Cauchy's integral formula</h><h>extensions of</h></idx>
        <me>
          f^{(k)} (w) \ = \ \frac{k!}{2 \pi i} \int_\gg \frac{ f(z) }{
          (z-w)^{k+1} } \, \diff{z} \, 
        </me>.
      </p>
    </statement>
  </corollary>
  <p>
    <xref ref="cauchyformula3"/>
    combined with our often-used
    <xref ref="intprop"/>(<xref text="local" ref="int4"></xref>)
    gives an inequality which is often called
    <em>Cauchy's Estimate</em>:
    <idx><h>Cauchy's estimate</h></idx>
  </p>
  <corollary xml:id="cauchyestimate">
    <statement>
      <p>
        Suppose <m>f</m> is holomorphic in <m>D[w,R]</m> and
        <m>|f(z)| \leq M</m> for all <m>z \in D[w,R]</m>.
        Then
        <me>
          \left| f^{(k)} (w) \right| \ \leq \ \frac{ k! \, M }{ R^k } \,
        </me>.
      </p>
    </statement>
  </corollary>
  <proof>
    <p>
      Let <m>r\lt R</m>.
      By <xref ref="cauchyformula3"/>
      and <xref ref="intprop"/>(<xref text="local" ref="int4"></xref>),
      <md>
        <mrow>\left| f^{(k)} (w) \right| \ \amp = \ \left| \frac{k!}{2
        \pi i} \int_{ C[w,r] } \frac{ f(z) }{ (z-w)^{k+1} } \,
        \diff{z} \right| \
        </mrow>
        <mrow> \amp \leq \ \frac{k!}{2 \pi} \max_{z \in C[w,r]
        } \left| \frac{ f(z) }{ (z-w)^{k+1} } \right| \length ( C[w,r]
        )</mrow> 
        <mrow>\amp \leq \ \frac{k!}{2 \pi} \, \frac{ M }{ r^{k+1} } \,
        2 \pi r
        </mrow>
        <mrow>\amp \ = \ \frac{ k! \, M }{ r^k } \, </mrow> 
      </md>.
    </p>
    <p>
      The statement now follows since <m>r</m> can be chosen
      arbitrarily close to <m>R</m>. 
    </p>
  </proof>
  <p>
    A key aspect of this section is worth emphasizing:
    namely, we have developed an alternative characterization of what
    it means for a function to be holomorphic. 
    In <xref ref="functionchapter"/>,
    we defined a function to be <em>holomorphic</em>
    in a region <m>G</m> if it is differentiable at each point <m>z_0 \in G</m>.
    We now define what it means for a function to be
    <em>analytic</em> in <m>G</m>.
  </p>
  <definition>
    <statement>
      <p>
        Let <m>f: G \to \C</m> and <m>z_0 \in G</m>.
        If there exist <m>R>0</m> and
        <m>c_0, c_1, c_2, \ldots \in \C</m> such that the power series
        <me>
          \s c_k (z-z_0)^k
        </me>
        converges in <m>D[z_0, R]</m> and agrees with <m>f(z)</m> in
        <m>D[z_0, R]</m>, 
        then <m>f</m> is <em>analytic at</em>
        <m>z_0</m>.
        <idx><h>analytic</h></idx>
        We call <m>f</m> <em>analytic in</em>
        <m>G</m> if <m>f</m> is analytic at each point
        in <m>G</m>. 
      </p>
    </statement>
  </definition>
  <p>
    What we have proved in this section can be summed up as follows:
  </p>
  <theorem>
    <statement>
      <p>
        For any region <m>G</m>,
        the class of all analytic functions in <m>G</m> coincides with
        the class of all holomorphic functions in <m>G</m>. 
      </p>
    </statement>
  </theorem>
  <p>
    While the terms <em>holomorphic</em> and <em>analytic</em>
    do not always mean the same thing,
    in the study of complex analysis they do and are frequently used
    interchangeably. 
  </p>
</section>
