<section xml:id="sec_exptrigfcts">
  <title>Exponential and Trigonometric Functions</title>
  <p>
    To define the complex exponential function,
    we once more borrow concepts from calculus,
    namely the real exponential function<fn>
    How to define the real exponential function is a nontrivial question.
    Our preferred way to do this is through a power series:
    <m>e^x = \sum_{k \geq 0} \frac 1 {k!} x^k</m>.
    In light of this definition,
    you might think we should have simply defined the complex exponential function through a complex power series.
    In fact, this is possible (and an elegant definition);
    however, one of the promises of this book is to introduce complex power series as late as possible.
    We agree with those readers who think that we are cheating at this point,
    as we borrow the concept of a (real) power series to define the real exponential function.
    </fn> and the real sine and cosine,
    and we finally make sense of the notation <m>e^{it} = \cos t + i \sin t</m>.
        <idx><h>function</h><h>exponential</h></idx>
  </p>
  <definition>
    <statement>
      <p>
        The <em>(complex) exponential function
            <idx><h>exponential function</h></idx>
        </em> is <m>\exp: \C \to \C</m>,
        defined for <m>z=x+iy</m> as
        <me>
          \exp(z) \ := \ e^x \left( \cos y + i \sin y \right) \= e^x e^{iy}
        </me>.
      </p>
    </statement>
  </definition>
  <p>
    This definition seems a bit arbitrary.
    Our first justification is that all exponential rules
        <idx><h>exponential rules</h></idx>
    that we are used to from real numbers carry over to the complex case.
    They mainly follow from <xref ref="easyexp">Proposition</xref>
    and are collected in the following.
  </p>
  <proposition xml:id="expproperties">
    <statement>
      <p>
        For all <m>z, z_1, z_2 \in \C</m>,
        <ol marker="a">
          <li>
            <p>
              <m>\exp \left( z_1 \right) \exp \left( z_2 \right) = \exp \left( z_1 + z_2 \right)</m>
            </p>
          </li>
          <li>
            <p>
              <m>\frac 1 {\exp \left( z \right)} = \exp \left( -z \right)</m>
            </p>
          </li>
          <li xml:id="expperiodic">
            <p>
              <m>\exp \left( z + 2 \pi i \right) = \exp \left( z \right)</m>
            </p>
          </li>
          <li>
            <p>
              <m>\left| \exp \left( z \right) \right| = \exp \left( \Re z \right)</m>
            </p>
          </li>
          <li>
            <p>
              <m>\exp(z) \ne 0</m>
            </p>
          </li>
          <li xml:id="expder">
            <p>
              <m>\frac{ d }{ d z } \exp \left( z \right) = \exp \left( z \right)</m>.
            </p>
          </li>
        </ol>
      </p>
    </statement>
  </proposition>
  <p>
    <xref ref="expperiodic">Identity</xref>
    is very special and has no counterpart for the real exponential function.
    It says that the complex exponential function is <em>periodic
        <idx><h>periodic</h></idx>
    </em> with period <m>2 \pi i</m>.
    This has many interesting consequences;
    one that may not seem too pleasant at first sight is the fact that the complex exponential function is not one-to-one.
  </p>
  <p>
    <xref ref="expder">Identity</xref> is not only remarkable,
    but we invite you to meditate on its proof below;
    it gives a strong indication that our definition of <m>\exp</m> is reasonable.
    We also note that <xref ref="expder"></xref>
    implies that <m>\exp</m> is entire.
  </p>
  <p>
    We leave the proof of <xref ref="expproperties">Proposition</xref>
    as <xref ref="ex_expproperties">Exercise</xref> but give one sample.
  </p>
  <proof>
    <p>
      The partial derivatives of <m>f(z) = \exp(z)</m> are
      <me>
        \fderiv fx \= e^x \left( \cos y + i \sin y \right) \qquad \text{ and }  \qquad \fderiv fy \= e^x \left( -\sin y + i \cos y \right)
      </me>.
    </p>
    <p>
      They are continuous in <m>\C</m> and satisfy the Cauchy<ndash/>Riemann equation<nbsp/><xref ref="complexcr"/>:
      <me>
        \fderiv fx(z) \= -i \, \fderiv fy(z)
      </me>
      for all <m>z \in \C</m>.
      Thus <xref ref="cre">Theorem</xref>
      says that <m>f(z) = \exp(z)</m> is entire with derivative
      <me>
        f'(z) \= \fderiv fx(z) \= \exp(z) \, . \qedhere
      </me>
    </p>
  </proof>
  <p>
    We should make sure that the complex exponential function specializes to the real exponential function for real arguments:
    indeed, if <m>z = x \in \R</m> then
    <me>
      \exp(x) \= e^x \left( \cos 0 + i \sin 0 \right) \= e^x
    </me>.
  </p>
  <figure>
    <caption>Image properties of the exponential function.</caption>
    <me>
      \figureinput Rtex/expimage
    </me>
  </figure>
  <p>
    The trigonometric functions
        <idx><h>trigonometric functions</h></idx>
    <mdash/>sine,
        <idx><h>sine</h></idx>
    cosine,
        <idx><h>cosine</h></idx>
    tangent,
        <idx><h>tangent</h></idx>
    cotangent,
        <idx><h>cotangent</h></idx>
    etc.<mdash/>also have complex analogues;
    however, they do not play the same prominent role as in the real case.
    In fact, we can define them as merely being special combinations of the exponential function.
        <idx><h>function</h><h>trigonometric</h></idx>
  </p>
  <definition>
    <statement>
      <p>
        The <em>(complex) sine</em> and
        <em>cosine</em> are defined as
        <me>
          \sin z \ := \ \tfrac{1}{2i} \left( \exp (iz) - \exp (-iz) \right) \qquad \text{ and }  \qquad \cos z \ := \ \tfrac 1 2 \left( \exp (iz) + \exp (-iz) \right)\,
        </me>,
        respectively.
        The <em>tangent</em> and <em>cotangent</em> are defined as
        <me>
          \tan z \ := \ \frac{ \sin z }{ \cos z } \= -i \, \frac{ \exp (2iz) - 1 }{ \exp (2iz) + 1 } \qquad \text{ and }  \qquad \cot z \ := \ \frac{ \cos z }{ \sin z } \= i \, \frac{ \exp (2iz) + 1 }{ \exp (2iz) - 1 } \,
        </me>,
        respectively.
      </p>
    </statement>
  </definition>
  <p>
    Note that to write tangent and cotangent in terms of the exponential function,
    we used the fact that <m>\exp(z) \exp(-z) = \exp(0) = 1</m>.
    Because <m>\exp</m> is entire,
    so are <m>\sin</m> and <m>\cos</m>.
  </p>
  <p>
    As with the exponential function,
    we should make sure that we're not redefining the real sine and cosine:
    if <m>z = x \in \R</m> then
    <me>
      \sin z \= \tfrac{1}{2i} \left( \exp (ix) - \exp (-ix) \right) \= \tfrac{1}{2i} \left( \cos x + i \sin x - \cos(-x) - i \sin(-x) \right) \= \sin x \,
    </me>.
  </p>
  <p>
    A similar calculation holds for the cosine.
    Not too surprisingly,
    the following properties follow mostly from <xref ref="expproperties">Proposition</xref>.
  </p>
  <proposition xml:id="trigproperties">
    <statement>
      <p>
        For all <m>z, z_1, z_2 \in \C</m>,
        <md>
          <mrow>\sin (-z) \amp = - \sin z \amp \cos (-z) \amp = \cos z</mrow>
          <mrow>\sin (z + 2 \pi) \amp = \sin z \amp \cos (z + 2 \pi) \amp = \cos z</mrow>
          <mrow>\tan (z + \pi) \amp = \tan z \amp \cot (z + \pi) \amp = \cot z</mrow>
          <mrow>\sin (z + \tfrac \pi 2) \amp = \cos z \amp \cos (z + \tfrac \pi 2) \amp = -\sin z</mrow>
          <mrow>\sin \left( z_1 + z_2 \right) \amp = \sin z_1 \cos z_2 + \cos z_1 \sin z_2 \qquad \amp \cos \left( z_1 + z_2 \right) \amp = \cos z_1 \cos z_2 - \sin z_1 \sin z_2</mrow>
          <mrow>\cos^2 z + \sin^2 z \amp = 1 \amp  \cos^2 z-\sin^2 z \amp = \cos(2z)</mrow>
          <mrow>\frac{ d }{ \diff{z} } \sin z \amp = \cos z \amp \frac{ d }{ \diff{z} } \cos z \amp = - \sin z \, </mrow>
        </md>.
      </p>
    </statement>
  </proposition>
  <p>
    Finally, one word of caution:
    unlike in the real case,
    the complex sine and cosine are
    <em>not</em> bounded<mdash/>consider,
    for example, <m>\sin (iy)</m> as <m>y \to \pm \infty</m>.
  </p>
  <p>
    We end this section with a remark on hyperbolic trig functions.
        <idx><h>hyperbolic trig functions</h></idx>
    The <em>hyperbolic sine</em>,
    <em>cosine</em>, <em>tangent</em>,
    and <em>cotangent</em> are defined as in the real case:
  </p>
  <definition>
    <statement>
      <md>
        <mrow>\sinh z \= \tfrac 1 {2} \left( \exp (z) - \exp (-z) \right) \qquad
        \amp \qquad \cosh z \= \tfrac 1 2 \left( \exp (z) + \exp (-z) \right)</mrow>
        <mrow>\tanh z \= \frac{ \sinh z }{ \cosh z } \= \frac{ \exp (2z) - 1 }{ \exp (2z) + 1 } \qquad
        \amp \qquad \coth z \= \frac{ \cosh z }{ \sinh z } \= \frac{ \exp (2z) + 1 }{ \exp (2z) - 1 } \, </mrow>
      </md>.
    </statement>
  </definition>
  <p>
    As such, they are yet more special combinations of the exponential function.
    They still satisfy the identities you already know, e.g.,
    <me>
      \frac{d}{\diff{z}} \sinh z \= \cosh z \qquad \text{ and }  \qquad \frac{d}{\diff{z}} \cosh z \= \sinh z \,
    </me>.
  </p>
  <p>
    Moreover, they are related to the trigonometric functions via
    <me>
      \sinh (iz) \= i \sin z \qquad \text{ and }  \qquad \cosh (iz) \= \cos z \,
    </me>.
  </p>
</section>